add a generation to each reference
I changed the naming conventions to better distinguish locations that
are used for references and those that are nodes in the store
graph. Only reference locations use 'r', and nodes use 'j, k, l, n'.

theories/persistent/pstore_1.v
@@ -22,14 +22,6 @@ From zoo.persistent Require Export
 From zoo Require Import
   options.
 
-#[local] Definition generation :=
-  nat.
-
-Implicit Types l : location.
-Implicit Types v t s : val.
-Implicit Types σ : gmap location val.
-Implicit Types gen : generation.
-
 #[local] Notation "'root'" := (
   in_type "t" 0
 )(in custom zoo_field
@@ -41,6 +33,10 @@ Implicit Types gen : generation.
 
 #[local] Notation "'sref_value'" := (
   in_type "sref" 0
+)(in custom zoo_field
+).
+#[local] Notation "'sref_gen'" := (
+  in_type "sref" 1
 )(in custom zoo_field
 ).
 
@@ -75,7 +71,7 @@ Definition pstore_create : val :=
 
 Definition pstore_ref : val :=
   λ: "t" "v",
-    { "v" }.
+    { "v"; #0 }.
 
 Definition pstore_get : val :=
   λ: "t" "r",
@@ -84,8 +80,9 @@ Definition pstore_get : val :=
 Definition pstore_set : val :=
   λ: "t" "r" "v",
     let: "root" := ref §Root in
-    "t".{root} <- ‘Diff{ "r", "r".{sref_value}, "root" } ;;
+    "t".{root} <- ‘Diff{ "r", "r".{sref_value}, "r".{sref_gen}, "root" } ;;
     "r" <-{sref_value} "v" ;;
+    "r" <-{sref_gen} "t".{gen} ;;
     "t" <-{root} "root".
 
 Definition pstore_capture : val :=
@@ -99,7 +96,7 @@ Definition pstore_collect : val :=
     match: !"node" with
     | Root =>
         ("node", "acc")
-    | Diff <> <> "node'" =>
+    | Diff <> <> <> "node'" =>
         "pstore_collect" "node'" ‘Cons{ "node", "acc" }
     end.
 Definition pstore_revert : val :=
@@ -111,10 +108,11 @@ Definition pstore_revert : val :=
         match: !"node'" with
         | Root =>
             Fail
-        | Diff "r" "v" "node_" =>
+        | Diff "r" "v" "gen" "node_" =>
             assert ("node_" = "node") ;;
-            "node" <- ‘Diff{ "r", "r".{sref_value}, "node'" } ;;
+            "node" <- ‘Diff{ "r", "r".{sref_value}, "r".{sref_gen}, "node'" } ;;
             "r" <-{sref_value} "v" ;;
+            "r" <-{sref_gen} "gen";;
             "pstore_revert" "node'" "seg"
         end
     end.
@@ -128,14 +126,14 @@ Definition pstore_restore : val :=
     if: "t" ≠ "s".<snap_store> then (
       Fail
     ) else (
-      let: "root" := "s".<snap_root> in
-      match: !"root" with
+      let: "snaproot" := "s".<snap_root> in
+      match: !"snaproot" with
       | Root =>
           ()
-      | Diff <> <> <> =>
-          pstore_reroot "root" ;;
+      | Diff <> <> <> <> =>
+          pstore_reroot "snaproot" ;;
           "t" <-{gen} #1 + "s".<snap_gen> ;;
-          "t" <-{root} "root"
+          "t" <-{root} "snaproot"
       end
     ).
 
@@ -801,13 +799,13 @@ Section graph.
   Definition undo_graph (g : graph A B) (xs ys : list (A * B * A)) : graph A B :=
     list_to_set ys ∪ g ∖ list_to_set xs.
 
-  Lemma undo_path g r xs rs ys :
-    path g rs xs r ->
+  Lemma undo_path g j xs k ys :
+    path g k xs j ->
     mirror xs ys ->
-    path (undo_graph g xs ys) r ys rs.
+    path (undo_graph g xs ys) j ys k.
   Proof.
     intros Hxs Hxsys.
-    enough (path (list_to_set ys) r ys rs) as Pys.
+    enough (path (list_to_set ys) j ys k) as Pys.
     { eapply path_weak.
     - eapply Pys.
     - unfold undo_graph; set_solver. }
@@ -923,23 +921,25 @@ End graph.
 (* Define apply_diffl, a function applying a list of diff. *)
 
 Section adiffl.
-  Notation diff := (
+  Context {V : Type}.
+
+  #[local] Notation diff := (
     (* location and its old value *)
-    location*val
+    location * V
   )%type.
 
-  Definition apply_diffl (ds:list diff) (σ:gmap location val) : gmap location val :=
-    foldr (fun '(l,v) σ => <[l:=v]> σ) σ ds.
+  Definition apply_diffl (ds:list diff) (σ:gmap location V) : gmap location V :=
+    foldr (fun '(l,w) (σ:gmap location V) => <[l:=w]> σ) σ ds.
 
-  Lemma dom_apply_diffl ds σ :
+  Lemma dom_apply_diffl ds (σ:gmap location V) :
     dom (apply_diffl ds σ) = dom σ ∪ (list_to_set ds.*1).
   Proof.
     induction ds as [|(?&?)]; set_solver.
   Qed.
 
-  Lemma apply_diffl_insert_ne ds l v σ :
+  Lemma apply_diffl_insert_ne ds l (w : V) (σ : gmap location V) :
     l ∉ ds.*1 ->
-    apply_diffl ds (<[l:=v]> σ) = <[l:=v]> (apply_diffl ds σ).
+    apply_diffl ds (<[l:=w]> σ) = <[l:=w]> (apply_diffl ds σ).
   Proof.
     induction ds as [|(?&?)].
     { intros ?. reflexivity. }
@@ -947,25 +947,25 @@ Section adiffl.
       rewrite insert_commute //. set_solver. }
   Qed.
 
-  Lemma apply_diffl_app ds ds' σ :
+  Lemma apply_diffl_app ds ds' (σ : gmap location V) :
     apply_diffl (ds++ds') σ = apply_diffl ds (apply_diffl ds' σ).
   Proof.
     rewrite /apply_diffl foldr_app //.
   Qed.
 
-  Lemma apply_diffl_snoc xs l v σ :
-    apply_diffl (xs ++ [(l,v)]) σ = apply_diffl xs (<[l:=v]> σ).
+  Lemma apply_diffl_snoc xs l w (σ : gmap location V) :
+    apply_diffl (xs ++ [(l,w)]) σ = apply_diffl xs (<[l:=w]> σ).
   Proof.
     rewrite apply_diffl_app //.
   Qed.
 
-  Lemma apply_diffl_cons l v xs σ :
-    apply_diffl ((l,v)::xs) σ = <[l:=v]> (apply_diffl xs σ).
+  Lemma apply_diffl_cons l w xs (σ : gmap location V) :
+    apply_diffl ((l,w)::xs) σ = <[l:=w]> (apply_diffl xs σ).
   Proof.
     done.
   Qed.
 
-  Lemma apply_diffl_included xs σ1 σ2 :
+  Lemma apply_diffl_included xs (σ1 σ2 : gmap location V) :
     σ1 ⊆ σ2 ->
     apply_diffl xs σ1 ⊆ apply_diffl xs σ2.
   Proof.
@@ -975,9 +975,52 @@ Section adiffl.
 End adiffl.
 
 (* ------------------------------------------------------------------------ *)
-(* Proof. *)
+(* Invariants. *)
 
-Notation snapshot_model := (location * gmap location val * generation)%type.
+Definition ref_loc := location.
+Definition node_loc := location.
+Definition generation := nat.
+
+Notation node_map V := (gmap node_loc V).
+Notation ref_map V := (gmap ref_loc V).
+Notation node_graph V := (graph node_loc V).
+
+Notation mapping := (ref_map val).
+
+Definition reference_model := (val * generation)%type.
+
+Definition snapshot_model := (node_loc * mapping * generation)%type.
+Notation snapshots_model := (gset snapshot_model).
+
+Definition mapping_diff := (ref_loc * val)%type.
+Definition ref_diff := (ref_loc * reference_model)%type.
+Definition ref_diff_edge := (node_loc * ref_diff * node_loc)%type.
+
+Notation graph_store := (node_graph ref_diff).
+Notation node_generations := (node_map generation).
+Notation map_model := (node_map mapping).
+
+Implicit Types j k l n root snaproot : node_loc.
+Implicit Types r : ref_loc.
+Implicit Types v t s : val.
+Implicit Types w : reference_model.
+Implicit Types σ : mapping.
+Implicit Types gen snapgen refgen : generation.
+
+Implicit Types g h : graph_store.
+Implicit Types M : map_model.
+Implicit Types G : node_generations.
+Implicit Types C : snapshots_model.
+
+Implicit Types ρv : ref_map val.
+Implicit Types ρg : ref_map generation.
+
+
+Definition vchange_of_edge : ref_diff_edge -> ref_loc * val :=
+  fun '(j, (r, (v, gen)), k) => (r, v).
+
+Definition gchange_of_edge : ref_diff_edge -> ref_loc * generation :=
+  fun '(j, (r, (v, gen)), k) => (r, gen).
 
 Class PstoreG Σ `{zoo_G : !ZooG Σ} := {
   #[local] pstore_G_set_G :: MonoSetG Σ snapshot_model ;
@@ -996,51 +1039,30 @@ Qed.
 Section pstore_G.
   Context `{pstore_G : PstoreG Σ}.
 
-  Notation diff := (
-    (* location and its old value. *)
-    location*val
-  )%type.
-  Notation graph_store := (
-    graph location diff
-  ).
-  Notation map_model := (
-    gmap location (gmap location val)
-  ).
-  Notation generation_model := (
-    gmap location generation
-  ).
-  Notation snapshots_model := (
-    gset snapshot_model
-  ).
-
-  Implicit Types g h : graph_store.
-  Implicit Types M : map_model.
-  Implicit Types C : snapshots_model.
-  Implicit Types G : generation_model.
-
   Definition correct_path_diff (M:map_model) (g:graph_store) :=
-    forall r1 ds r2 σ1 σ2,
-      path g r1 ds r2 -> M !! r1 = Some σ1 -> M !! r2 = Some σ2 ->
-      σ1 = (apply_diffl (proj2 <$> ds) σ2).
+    forall n1 (ds : list ref_diff_edge) n2 σ1 σ2,
+      path g n1 ds n2 -> M !! n1 = Some σ1 -> M !! n2 = Some σ2 ->
+      σ1 = (apply_diffl (vchange_of_edge <$> ds) σ2).
 
-  Record store_inv (M:map_model) (G:generation_model) (g:graph_store) (r:location) (σ σ0:gmap location val) :=
-    { si1M : dom M = vertices g ∪ {[r]};
+  Record store_inv (M:map_model) (G:node_generations) (g:graph_store) (root:node_loc) σ ρv :=
+    { si1M : dom M = vertices g ∪ {[root]};
       si1G : dom M = dom G;
-      si2 : σ ⊆ σ0;
-      si3 : M !! r = Some σ0 ;
+      si2 : σ ⊆ ρv;
+      si3 : M !! root = Some ρv ;
       si4 : correct_path_diff M g
     }.
 
-  Definition locations_of_edges_in g (X:gset location) :=
-    forall (r:location) l v r', edge g r (l,v) r' -> l ∈ X.
+  Definition references_in g (X:gset ref_loc) :=
+    forall n r w n', edge g n (r,w) n' -> r ∈ X.
 
-  Record coherent (M:map_model) (σ0:gmap location val) (g:graph_store) :=
-    { coh1 : forall r σ, M !! r = Some σ -> dom σ = dom σ0;
-      coh2 : locations_of_edges_in g (dom σ0);
+  Record coherent (M:map_model) ρv ρg g :=
+    { coh1 : forall n σ, M !! n = Some σ -> dom σ = dom ρv;
+      coh2 : references_in g (dom ρv);
+      coh3 : dom ρv = dom ρg;
     }.
 
-  Definition captured C l :=
-    exists σ gen, (l, σ, gen) ∈ C.
+  Definition captured C n :=
+    exists σ gen, (n, σ, gen) ∈ C.
 
   (* TODO include in stdpp ?
      https://gitlab.mpi-sws.org/iris/stdpp/-/issues/209 *)
@@ -1078,33 +1100,33 @@ Section pstore_G.
   Definition at_most_one_child g k :=
     forall k1 k2, has_edge g k1 k -> has_edge g k2 k -> k1 = k2.
 
-  Definition topology_inv g M C r :=
+  Definition topology_inv g M C root :=
     (* If a node is not captured, then:
        - if it is the current root, it has no children
        - otherwise it has at most one child *)
     forall k, k ∈ dom M -> not (captured C k) ->
-      ((k = r) -> no_succ g k)
+      ((k = root) -> no_succ g k)
       /\
       (at_most_one_child g k)
     .
 
-  Lemma topology_domM_transport : forall g M M' C r,
-    dom M = dom M' -> topology_inv g M C r -> topology_inv g M' C r.
+  Lemma topology_domM_transport : forall g M M' C root,
+    dom M = dom M' -> topology_inv g M C root -> topology_inv g M' C root.
   Proof.
-    intros g M M' C r H Htop.
+    intros g M M' C root H Htop.
     intros k Hk.
     rewrite <- H in Hk.
     exact (Htop k Hk).
   Qed.
 
-  Definition history_inv g r h orig :=
+  Definition history_inv g root h orig :=
     exists xs ys,
-      path g orig xs r /\
+      path g orig xs root /\
       mirror xs ys /\
       h ≡ undo_graph g xs ys.
 
-  Lemma history_vertices g r h orig :
-    history_inv g r h orig ->
+  Lemma history_vertices g root h orig :
+    history_inv g root h orig ->
     vertices g = vertices h.
   Proof.
     intros (xs & ys & Pxs & Mxsys & Hundo).
@@ -1113,17 +1135,17 @@ Section pstore_G.
     eapply path_all_in; eauto.
   Qed.
 
-  Lemma history_vertices_have_a_generation M C G g r σ σ0 h orig :
-    store_inv M G g r σ σ0 ->
-    history_inv g r h orig ->
+  Lemma history_vertices_have_a_generation M C G g root σ ρv h orig :
+    store_inv M G g root σ ρv ->
+    history_inv g root h orig ->
     forall k, k ∈ vertices h ->
     exists kgen, G !! k = Some kgen.
   Proof.
     intros Hstore_inv Histo_inv k Hk.
-    rewrite -(history_vertices g r h orig) in Hk; eauto.
+    rewrite -(history_vertices g root h orig) in Hk; eauto.
     destruct Hstore_inv.
     assert (k ∈ dom G) as HkG by set_solver.
-    apply elem_of_dom; eauto.
+    eapply elem_of_dom; eauto.
   Qed.
 
   (* The relation between the generation of a node and the generational of
@@ -1131,7 +1153,7 @@ Section pstore_G.
      - if the parent is captured, the generation was incremented by the capture(s)
        so the child has a strictly greater generation
      - otherwise they have the same generation. *)
-  Definition gen_succ_rel C G (child_gen : generation) (parent : location) :=
+  Definition gen_succ_rel C G (child_gen : generation) (parent : node_loc) :=
     match G !! parent with
     | None => False
     | Some parent_gen =>
@@ -1141,14 +1163,14 @@ Section pstore_G.
         child_gen = parent_gen
     end.
 
-  Definition global_gen_inv h C G r store_gen :=
+  Definition global_gen_inv h C G root store_gen :=
     (* All nodes respect the parent-child generation relation. *)
     (forall k gk l, has_edge h k l -> G !! k = Some gk ->
       gen_succ_rel C G gk l)
     /\
     (* The global generation of the store would be a valid generation
        for a child of the current root. *)
-    (gen_succ_rel C G store_gen r).
+    (gen_succ_rel C G store_gen root).
 
   Definition snapshot_inv M C G l σ snap_gen :=
     exists σ',
@@ -1171,20 +1193,32 @@ Section pstore_G.
   #[local] Definition pstore_map_elem γ l σ gen :=
     mono_set_elem γ (l, σ, gen).
 
-  Lemma extract_unaliased (g : graph_store) :
-    ([∗ set] '(r, (l, v), r') ∈ g, r ↦ ’Diff{ #(l : location), v, #(r' : location) }) -∗
-    ⌜unaliased g⌝.
+
+  (* FIXME: I don't know how to unfold notations in spatial hypotheses,
+     so let's just make those notations for now. *)
+  Notation ref_values ρv :=
+    ([∗ map] r ↦ v ∈ ρv,
+      r.[sref_value] ↦ v)%I.
+  Notation ref_generations ρg :=
+    ([∗ map] r ↦ refgen ∈ ρg,
+      r.[sref_gen] ↦ #(refgen : generation))%I.
+  Notation diff_nodes g :=
+    ([∗ set] '(j, (r, (v, refgen)), k) ∈ g,
+      j ↦ ’Diff{ #(r : ref_loc), v, #(refgen : generation), #(k : node_loc) })%I.
+
+  Lemma extract_unaliased g : diff_nodes g -∗ ⌜unaliased g⌝.
   Proof.
-    iIntros "Hg" (???????).
-    destruct_decide (decide (a0 = a2 ∧ a1 = a3)); first done.
-    rewrite (big_sepS_delete _ _ (a, a0, a1)); first set_solver.
-    rewrite (big_sepS_delete _ _ (a, a2, a3)); first set_solver.
-    iDestruct "Hg" as "(?&?&_)". destruct a0,a2.
+    iIntros "Hg" (j d1 k1 d2 k2 H1 H2).
+    destruct_decide (decide (d1 = d2 ∧ k1 = k2)); first done.
+    rewrite (big_sepS_delete _ _ (j, d1, k1)); first set_solver.
+    rewrite (big_sepS_delete _ _ (j, d2, k2)); first set_solver.
+    destruct d1 as (r1, (v1, gen1)), d2 as (r2, (v2, gen2)).
+    iDestruct "Hg" as "(H1 & H2 & _)".
     iDestruct (pointsto_ne with "[$][$]") as "%". congruence.
   Qed.
 
-  Lemma generations_decrease_along_history_edge h M C G r store_gen k l gk gl :
-    global_gen_inv h C G r store_gen ->
+  Lemma generations_decrease_along_history_edge h M C G root store_gen k l (gk gl : generation) :
+    global_gen_inv h C G root store_gen ->
     has_edge h k l ->
     G !! k = Some gk ->
     G !! l = Some gl ->
@@ -1197,8 +1231,8 @@ Section pstore_G.
     destruct_decide (decide (captured C l)); lia.
   Qed.
 
-  Lemma generations_decrease_along_history_path h M C G r store_gen na xs nb gena genb :
-    global_gen_inv h C G r store_gen ->
+  Lemma generations_decrease_along_history_path h M C G root store_gen na xs nb gena genb :
+    global_gen_inv h C G root store_gen ->
     vertices h ⊆ dom G ->
     path h na xs nb ->
     G !! na = Some gena ->
@@ -1239,30 +1273,32 @@ Section pstore_G.
       ⌜snapshots_inv M C G⌝ ∗ meta t0 nroot γ ∗ pstore_map_auth γ C.
 
   #[local] Definition pstore (t:val) (σ:gmap location val) : iProp Σ :=
-    ∃ (t0 r orig:location) gen
-      (σ0:gmap location val) (* the global map, with all the points-to ever allocated *)
+    ∃ (t0 root orig:location) gen
+      (ρv:ref_map val) (* the value of each reference *)
+      (ρg:ref_map generation) (* the generation of each reference *)
       (g:graph_store) (* the current graph *)
       (h:graph_store) (* the historic graph *)
       (M:map_model) (* the map model, associating to each node its model *)
       (C:snapshots_model) (* the subset of nodes captured as snapshots *)
-      (G:generation_model) (* the generation of each node *)
+      (G:node_generations) (* the generation of each node *)
       ,
     ⌜t=#t0 /\
-     store_inv M G g r σ σ0 /\
-     topology_inv g M C r /\
-     history_inv g r h orig /\
-     coherent M σ0 g /\
-     rooted_dag g r /\
-     global_gen_inv h C G r gen⌝ ∗
-    t0.[root] ↦ #r ∗
+     store_inv M G g root σ ρv /\
+     topology_inv g M C root /\
+     history_inv g root h orig /\
+     coherent M ρv ρg g /\
+     rooted_dag g root /\
+     global_gen_inv h C G root gen⌝ ∗
+    t0.[root] ↦ #root ∗
     t0.[gen] ↦ #gen ∗
-    r ↦ §Root ∗
+    root ↦ §Root ∗
     snapshots t0 M C G ∗
-    ([∗ map] l ↦ v ∈ σ0, l.[sref_value] ↦ v) ∗
-    ([∗ set] x ∈ g, let '(r,(l,v),r') := x in r ↦ ’Diff{ #(l : location), v, #(r' : location) }) .
+    ref_values ρv ∗
+    ref_generations ρg ∗
+    diff_nodes g.
 
   Definition open_inv : string :=
-    "[%t0 [%r [%orig [%gen [%σ0 [%g [%h [%M [%C [%G
+    "[%t0 [%root [%orig [%gen [%ρv [%ρg [%g [%h [%M [%C [%G
        ((-> &
          %Hinv &
          %Htopo &
@@ -1273,11 +1309,12 @@ Section pstore_G.
         ) &
         Ht0 &
         Hgen &
-        Hr &
+        Hroot &
         HC &
-        Hσ0 &
+        Hρv &
+        Hρg &
         Hg
-       )]]]]]]]]]]".
+       )]]]]]]]]]]]".
 
   Definition pstore_snapshot t s σ : iProp Σ :=
     ∃ γ (t0:location) l gen,
@@ -1304,12 +1341,15 @@ Section pstore_G.
   Proof.
     iIntros "%Φ _ HΦ".
     wp_rec.
-    wp_alloc r as "Hroot".
+    wp_alloc root as "Hroot".
     wp_record t0 as "Hmeta" "(Ht0 & Hgen & _)".
     iMod (mono_set_alloc ∅) as "[%γ ?]".
     iMod (meta_set _ _ _ nroot with "Hmeta") as "Hmeta"; first set_solver.
     iApply "HΦ". iModIntro.
-    iExists t0,r,r,0,∅,∅,∅,{[r := ∅]},∅,{[r := 0]}. iFrame.
+    iExists (* r0, root, orig, gen: *) t0, root, root, 0,
+            (* ρv, ρg, g, h: *) ∅, ∅, ∅, ∅,
+            (* M, C, G: *) {[root := ∅]}, ∅, {[root := 0]}.
+    iFrame.
     rewrite !big_sepM_empty big_sepS_empty !right_id.
     iSplitR.
     2:{ iExists γ. iFrame. iPureIntro. intros ??. set_solver. }
@@ -1320,14 +1360,14 @@ Section pstore_G.
       { set_solver. }
       { set_solver. }
       { rewrite lookup_insert //. }
-      { intros ????? Hr.
+      { intros ????? Hroot.
         rewrite !lookup_singleton_Some.
-        inversion Hr; set_solver. } }
+        inversion Hroot; set_solver. } }
     { (* topology_inv *)
       constructor.
-    - intro Hr; subst. intros l' (diff & Hedge).
+    - intro Hroot; subst. intros l' (diff & Hedge).
       set_solver.
-    - assert (k = r) by set_solver; subst.
+    - assert (k = root) by set_solver; subst.
       intros k1 k2 H1 H2.
       destruct H1; set_solver.
     }
@@ -1336,8 +1376,8 @@ Section pstore_G.
       split_and!; eauto; constructor.
     }
     { (* coherent *)
-      constructor.
-      { intros ??. rewrite lookup_singleton_Some. intros (->&->). reflexivity. }
+      constructor; eauto.
+      { intros ??. rewrite lookup_singleton_Some. intros (->&<-). reflexivity. }
       { intros ????. set_solver. } }
     { (* rooted_dag *)
       eauto using rooted_dag_empty. }
@@ -1347,7 +1387,7 @@ Section pstore_G.
       set_solver.
     - unfold gen_succ_rel.
       rewrite lookup_singleton.
-      { destruct_decide (decide (captured ∅ r)) as Hcap.
+      { destruct_decide (decide (captured ∅ root)) as Hcap.
       - unfold captured in Hcap.
         set_solver.
       - auto.
@@ -1355,14 +1395,40 @@ Section pstore_G.
     }
   Qed.
 
-  Lemma use_locations_of_edges_in g r xs r' X :
-    locations_of_edges_in g X ->
-    path g r xs r' ->
-    (list_to_set (proj2 <$> xs).*1) ⊆ X.
+  Lemma use_references_in g n ds n' X :
+    references_in g X ->
+    path g n ds n' ->
+    (list_to_set (vchange_of_edge <$> ds).*1) ⊆ X.
   Proof.
     intros He.
     induction 1; first set_solver.
+    destruct b as (r & v & gen).
     apply He in H. set_solver.
+  Qed.
+
+  Lemma use_r_in_dom {A B : Type} (m1 : ref_map A) (m2 : ref_map B) r (x : A) :
+    dom m1 ⊆ dom m2 ->
+    m1 !! r = Some x ->
+    exists (y : B), m2 !! r = Some y.
+  Proof.
+    intros Hdom Hσr.
+    assert (is_Some (m1 !! r)) as H by eauto.
+    rewrite -elem_of_dom in H.
+    apply Hdom in H.
+    rewrite elem_of_dom in H.
+    exact H.
+  Qed.
+
+  Lemma use_r_notin_dom {A B : Type} (m1 : ref_map A) (m2 : ref_map B) r :
+    dom m1 ⊆ dom m2 ->
+    m2 !! r = None ->
+    m1 !! r = None.
+  Proof.
+    intros Hdom H.
+    rewrite -not_elem_of_dom elem_of_dom.
+    intros (x & Hx).
+    destruct (use_r_in_dom m1 m2 r x Hdom) as (y & Hy); eauto.
+    naive_solver.
   Qed.
 
   Lemma pstore_ref_spec t σ v :
@@ -1370,34 +1436,40 @@ Section pstore_G.
       pstore t σ
     }}}
       pstore_ref t v
-    {{{ l,
-      RET #l;
-      ⌜l ∉ dom σ⌝ ∗
-      pstore t (<[l := v]> σ)
+    {{{ r,
+      RET #r;
+      ⌜r ∉ dom σ⌝ ∗
+      pstore t (<[r := v]> σ)
     }}}.
   Proof.
     iIntros (ϕ) open_inv. iIntros "HΦ".
 
-    wp_rec. wp_record l as "( Hl & _ )".
+    wp_rec. wp_record r as "( Hr & Hrgen & Hrest )".
 
     iApply "HΦ".
 
-    iAssert ⌜σ0 !! l = None⌝%I as %Hl0.
-    { rewrite -not_elem_of_dom. iIntros "%Hldom".
-      iDestruct (big_sepM_lookup with "Hσ0") as "( Hl_ & Hfoo & _ )".
-      { apply lookup_lookup_total_dom. exact Hldom. }
-      iDestruct (pointsto_ne with "Hl Hl_") as %?. done.
+    iAssert ⌜ρv !! r = None⌝%I as %Hρvr.
+    { rewrite -not_elem_of_dom elem_of_dom. iIntros "[%rv %Hrv]".
+      iDestruct (big_sepM_lookup with "Hρv") as "Hr'".
+      { eauto. }
+      iDestruct (pointsto_ne with "Hr Hr'") as %?. done.
     }
-    assert (σ !! l = None).
-    { eapply not_elem_of_dom. apply not_elem_of_dom in Hl0.  destruct Hinv as [_ _ X].
-      apply incl_dom_incl in X. set_solver. }
-    iDestruct (pointsto_ne with "Hl Hr") as %Hlr.
+    assert (ρg !! r = None) as Hρgr.
+    { destruct Hcoh; apply use_r_notin_dom with ρv; eauto.
+      rewrite coh6; eauto. }
+    assert (σ !! r = None).
+    { apply use_r_notin_dom with ρv; eauto.
+      apply incl_dom_incl. destruct Hinv; eauto. }
+
+    iDestruct (pointsto_ne with "Hr Hroot") as %Hlr.
 
     iModIntro. iSplitR. { iPureIntro. by eapply not_elem_of_dom. }
-    iExists t0,r,orig,gen, (<[l:=v]>σ0),g,h,((fun σ => <[l:=v]>σ)<$> M),C,G.
+    iExists (* r0, root, orig, gen: *) t0, root, orig, gen,
+            (* ρv, ρg, g, h: *) (<[r:=v]>ρv), (<[r:=0]>ρg), g, h,
+            (* M, C, G: *) ((fun σ => <[r:=v]>σ)<$> M),C,G.
 
-    rewrite big_sepM_insert //. iFrame "∗".
-    iSplitR "HC"; first (iPureIntro; split_and!; eauto).
+    do 2 rewrite big_sepM_insert //. iFrame "∗".
+    iSplitL "Hrest"; [ iPureIntro; split_and!; eauto | eauto ].
     { (* store_inv *)
       destruct Hinv as [X1 X2 X3 X4].
       constructor.
@@ -1405,16 +1477,16 @@ Section pstore_G.
       { rewrite dom_fmap_L; set_solver. }
       { eauto using gmap_included_insert. }
       { rewrite lookup_fmap X4 //. }
-      { intros r1 ds r2 σ1 σ2 Hr. rewrite !lookup_fmap. generalize Hr. intros Hreach.
-        intros Hr1 Hr2.
-        destruct (M !! r1) eqn:Hor1. 2:simpl in *; congruence.
-        inversion Hr1. subst.
-        destruct (M !! r2) eqn:Hor2. 2:simpl in *; congruence.
-        inversion Hr2. subst.
+      { intros l1 ds l2 σ1 σ2 Hl. rewrite !lookup_fmap. generalize Hl. intros Hreach.
+        intros Hl1 Hl2.
+        destruct (M !! l1) eqn:Hor1. 2:simpl in *; congruence.
+        inversion Hl1. subst.
+        destruct (M !! l2) eqn:Hor2. 2:simpl in *; congruence.
+        inversion Hl2. subst.
         destruct Hcoh as [Z1 Z2].
-        eapply use_locations_of_edges_in in Z2. 2:done.
+        eapply use_references_in in Z2. 2:done.
         rewrite apply_diffl_insert_ne.
-        { apply not_elem_of_dom in Hl0. set_solver. }
+        { apply not_elem_of_dom in Hρvr. set_solver. }
         { f_equal. eauto. } } }
     { (* topology_inv *)
       apply (topology_domM_transport g M).
@@ -1424,44 +1496,63 @@ Section pstore_G.
     { (* coherent *)
       destruct Hcoh as [X1 X2].
       constructor.
-      { intros r' ?. rewrite lookup_fmap. intros E.
-        destruct (M !! r') eqn:Hor. 2:simpl in *; congruence.
-        inversion E. subst. rewrite !dom_insert_L. set_solver. }
-      { intros. rewrite dom_insert_L. intros ??. set_solver. } }
-    { (* snapshots *)
+    - intros r' ?. rewrite lookup_fmap. intros E.
+      destruct (M !! r') eqn:Hor. 2:simpl in *; congruence.
+      inversion E. subst. rewrite !dom_insert_L. set_solver.
+    - intros. rewrite dom_insert_L. intros ??. set_solver.
+    - do 2 rewrite dom_insert_L; set_solver.
+    }
+    { (* snapshots_inv *)
       iDestruct "HC" as "[% (%Hsnap&?&?)]".
-      iExists _. iFrame. iPureIntro.
-      intros r' ? ? HC. apply Hsnap in HC. destruct HC as (x & Hx & ? & ?).
-      exists (<[l:=v]>x).
+      iExists γ. iFrame. iPureIntro.
+      intros snaproot ? ? HC. apply Hsnap in HC. destruct HC as (x & Hx & ? & ?).
+      exists (<[r:=v]>x).
       split_and!; eauto.
       - rewrite lookup_fmap Hx; eauto.
       - apply gmap_included_insert_notin; eauto.
         apply incl_dom_incl in H0. intros X. apply H0 in X.
         destruct Hcoh as [X1 X2]. apply X1 in Hx.
-        apply not_elem_of_dom in Hl0. set_solver. }
+        apply not_elem_of_dom in Hρvr. set_solver. }
   Qed.
 
-  Lemma pstore_get_spec {t σ l} v :
-    σ !! l = Some v →
+
+  Lemma use_r_in_σ {M G g root} σ ρv r v :
+    store_inv M G g root σ ρv ->
+    σ !! r = Some v ->
+    ρv !! r = Some v.
+  Proof.
+    intros Hinv Hr.
+    destruct Hinv.
+    pose proof (si5 r) as Hρr.
+    rewrite Hr in Hρr.
+    cbn in Hρr.
+    destruct (ρv !! r); naive_solver.
+  Qed.
+
+  Lemma pstore_get_spec {t σ r} v :
+    σ !! r = Some v →
     {{{
       pstore t σ
     }}}
-      pstore_get t #l
+      pstore_get t #r
     {{{
       RET v;
       pstore t σ
     }}}.
   Proof.
-    iIntros (Hl ϕ) open_inv. iIntros "HΦ".
+    iIntros (Hr ϕ) open_inv. iIntros "HΦ".
     wp_rec. iStep 4. iModIntro.
 
-    iDestruct (big_sepM_lookup_acc _ _ l v with "Hσ0") as "(Hl & Hclose)".
-    { destruct Hinv as [_ _ Hincl _ _].
-      specialize (Hincl l). rewrite Hl in Hincl. destruct (σ0!!l); naive_solver. }
+    assert (ρv !! r = Some v) as Hρv.
+    { eapply use_r_in_σ with σ; eauto. }
+
+    iDestruct (big_sepM_lookup_acc _ _ r v with "Hρv") as "(H & Hclose)"; eauto.
 
     wp_load. iStep. iModIntro.
 
-    iExists t0,r,orig,gen,σ0,g,h,M,C,G.
+    iExists (* r0, root, orig, gen: *) t0, root, orig, gen,
+            (* ρv, ρg, g, h: *) ρv, ρg, g, h,
+            (* M, C, G: *) M, C, G.
     iFrame.
     { iSplit.
     - iPureIntro.
@@ -1470,58 +1561,64 @@ Section pstore_G.
     }
   Qed.
 
-  Lemma pstore_set_spec t σ l v :
-    l ∈ dom σ →
+  Lemma pstore_set_spec t σ r v :
+    r ∈ dom σ →
     {{{
       pstore t σ
     }}}
-      pstore_set t #l v
+      pstore_set t #r v
     {{{
       RET ();
-      pstore t (<[l := v]> σ)
+      pstore t (<[r := v]> σ)
     }}}.
   Proof.
-    iIntros (Hl Φ) open_inv. iIntros "HΦ".
+    iIntros (Hr Φ) open_inv. iIntros "HΦ".
     wp_rec. iStep 8. iModIntro.
-    wp_alloc r' as "Hr'".
+    wp_alloc newroot as "Hnewroot".
 
-    assert (exists w, σ0 !! l = Some w) as (w&Hl0).
-    { apply elem_of_dom. destruct Hinv as [_ _ Hincl].
-      apply incl_dom_incl in Hincl.
-      set_solver. }
+    rewrite elem_of_dom in Hr.
+    destruct Hr as (old & Hold).
 
-    iDestruct (big_sepM_insert_acc with "Hσ0") as "( Hl & Hσ0 )"; first done.
-    wp_load. wp_load. wp_store. iStep 4. iModIntro.
-    wp_store. wp_store. iApply "HΦ".
+    assert (ρv !! r = Some old) as Hρr.
+    { eapply use_r_in_σ; eauto. }
+    destruct (use_r_in_dom ρv ρg r old) as (refgen & Hrefgen); eauto.
+    { destruct Hcoh. set_solver. }
 
-    iSpecialize ("Hσ0" with "[$]").
+    iDestruct (big_sepM_insert_acc with "Hρv") as "(Hv & Hρv)"; first done.
+    iDestruct (big_sepM_insert_acc with "Hρg") as "(Hrgen & Hρg)" ; first done.
+    wp_load. wp_load. wp_load. wp_store. wp_store. wp_load. wp_store. wp_store. iStep.
 
-    iAssert ⌜r ≠ r'⌝%I as %?.
-    { iClear "Ht0". iDestruct (pointsto_ne with "[$][$]") as %?. done. }
+    iSpecialize ("Hρv" with "[$]").
+    iSpecialize ("Hρg" with "[$]").
 
-    iAssert ⌜r' ∉ vertices g⌝%I as %Hr'.
-    { iIntros (Hr'). destruct Hgraph as [X1 X2].
-      apply X1 in Hr'. destruct Hr' as (?&Hr'). inversion Hr'; subst.
+    iAssert ⌜newroot ≠ root⌝%I as %?.
+    { iClear "Ht0". iDestruct (pointsto_ne with "Hnewroot Hroot") as %?. done. }
+
+    iAssert ⌜newroot ∉ vertices g⌝%I as %Hnewroot.
+    { iIntros (Hnewroot). destruct Hgraph as [X1 X2].
+      apply X1 in Hnewroot. destruct Hnewroot as (?&Hnewroot). inversion Hnewroot; subst.
       { done. }
-      { destruct b. iDestruct (big_sepS_elem_of with "[$]") as "?"; first done.
-        iDestruct (pointsto_ne r' r' with "[$][$]") as %?. congruence. } }
+      { destruct b. destruct r1. iDestruct (big_sepS_elem_of with "[$]") as "H"; first done.
+        iSimpl in "H".
+        iDestruct (pointsto_ne with "H Hnewroot") as %?. congruence. } }
 
     iModIntro.
-    iExists
-      t0,r',orig,gen,
-      (<[l:=v]> σ0),
-      ({[(r,(l,w),r')]} ∪ g),
-      ({[(r',(l,w),r)]} ∪ h),
-      (<[r':=<[l:=v]> σ0]>M),
-      C,
-      (<[r':=gen]>G).
+
+    set rdiff := (r, (old, refgen)).
+
+    iExists (* r0, root, orig, gen: *) t0, newroot, orig, gen,
+            (* ρv, ρg: *) (<[r:=v]>ρv), (<[r:=gen]>ρg),
+            (* g, h: *)   ({[(root, rdiff, newroot)]} ∪ g),
+                          ({[(newroot, rdiff, root)]} ∪ h),
+            (* M, C, G: *) (<[newroot:=<[r:=v]> ρv]>M), C, (<[newroot:=gen]>G).
+
     rewrite big_sepS_union.
-    { apply disjoint_singleton_l. intros ?. apply Hr'.
+    { apply disjoint_singleton_l. intros ?. apply Hnewroot.
       apply elem_of_vertices. eauto. }
-    rewrite big_sepS_singleton. iFrame "#∗".
+    rewrite big_sepS_singleton /rdiff. iFrame "#∗".
 
     iDestruct "HC" as "[% (%Hsnap&?&?)]".
-    { iSplitR; first (iPureIntro; split_and!; first done).
+    { iSplitR; [ iPureIntro; split_and!; first done | eauto ].
     - (* store_inv *)
       destruct Hinv as [X1 X2 X3 X4 X5].
       constructor.
@@ -1529,16 +1626,16 @@ Section pstore_G.
       { set_solver. }
       { apply gmap_included_insert. done. }
       { rewrite lookup_insert //. }
-      { intros r1 ds r2 σ1 σ2 Hreach.
-        destruct_decide (decide (r'=r1)).
+      { intros l1 ds l2 σ1 σ2 Hreach.
+        destruct_decide (decide (newroot = l1)).
         { subst. rewrite lookup_insert. inversion_clear 1.
           inversion Hreach.
           2:{ exfalso. subst. rewrite /edge elem_of_union in H0.
-              destruct H0; first set_solver. apply Hr'. apply elem_of_vertices. set_solver. }
+              destruct H0; first set_solver. apply Hnewroot. apply elem_of_vertices. set_solver. }
           subst.
           rewrite lookup_insert. inversion 1. done. }
         rewrite lookup_insert_ne //. intros E1.
-        destruct_decide (decide (r2=r')).
+        destruct_decide (decide (l2 = newroot)).
         { subst. rewrite lookup_insert. inversion 1. subst.
           apply path_add_inv_r in Hreach; try done.
           destruct Hreach as [(->&->)|(ds'&->&Hreach)].
@@ -1548,7 +1645,7 @@ Section pstore_G.
         { rewrite lookup_insert_ne //. intros. eapply X5; eauto.
           apply path_cycle_end_inv_aux in Hreach; eauto. } }
     - (* topology_inv *)
-      intros k Hk_dom Hk_cap.
+      intros k Hk_dom CAPk.
       { constructor.
       - (* no_succ *)
         intros Hk; subst.
@@ -1557,7 +1654,7 @@ Section pstore_G.
         rewrite elem_of_singleton in Hk'.
         { destruct Hk' as [ Hk' | Hk' ].
         - injection Hk'; intros; subst. auto.
-        - contradiction Hr'.
+        - contradiction Hnewroot.
           eapply left_vertex; eauto.
         }
       - (* at_most_one_child *)
@@ -1566,16 +1663,16 @@ Section pstore_G.
         rewrite -> elem_of_union in Hk2.
         { destruct Hk1; destruct Hk2.
         - set_solver.
-        - assert (k = r') by set_solver. subst.
-          contradiction Hr'. eapply right_vertex. eauto.
-        - assert (k = r') by set_solver. subst.
-          contradiction Hr'. eapply right_vertex. eauto.
+        - assert (k = newroot) by set_solver. subst.
+          contradiction Hnewroot. eapply right_vertex. eauto.
+        - assert (k = newroot) by set_solver. subst.
+          contradiction Hnewroot. eapply right_vertex. eauto.
         - assert (k ∈ dom M) as Hkm.
           { rewrite -> dom_insert in Hk_dom.
             rewrite -> elem_of_union in Hk_dom.
             { destruct Hk_dom as [ Hk_dom | Hk_dom ]; last assumption.
             - rewrite elem_of_singleton in Hk_dom; subst.
-              contradiction Hr'. eapply right_vertex. eauto.
+              contradiction Hnewroot. eapply right_vertex. eauto.
             }
           }
           apply (Htopo k); try eexists; eauto.
@@ -1583,8 +1680,8 @@ Section pstore_G.
       }
     - (* history_inv *)
       destruct Hist as (xs & ys & Hpath & Hmirror & Hhisto).
-      exists (xs ++ [(r, (l, w), r')]).
-      exists ((r', (l, w), r) :: ys).
+      exists (xs ++ [(root, rdiff, newroot)]).
+      exists ((newroot, rdiff, root) :: ys).
       { split_and!.
       - { apply path_snoc.
         - eapply path_weak; set_solver.
@@ -1602,46 +1699,48 @@ Section pstore_G.
         enough (
           g ∖ list_to_set xs
           ≡
-          ({[(r, (l, w), r')]} ∪ g) ∖ (list_to_set xs ∪ {[(r, (l, w), r')]})
+          ({[(root, rdiff, newroot)]} ∪ g) ∖ (list_to_set xs ∪ {[(root, rdiff, newroot)]})
         ) as Henough by (setoid_rewrite Henough; set_solver).
         rewrite difference_union_distr_l.
         setoid_replace
-          ({[(r, (l, w), r')]} ∖ (list_to_set xs ∪ {[(r, (l, w), r')]}) : graph_store)
+          ({[(root, rdiff, newroot)]} ∖ (list_to_set xs ∪ {[(root, rdiff, newroot)]}) : graph_store)
           with (∅ : graph_store) by set_solver.
         rewrite difference_union_distr_r.
         setoid_replace
-          (g ∖ {[(r, (l, w), r')]}) with g; first last.
+          (g ∖ {[(root, rdiff, newroot)]}) with g; first last.
         { apply difference_disjoint.
           unfold disjoint.
           intros tri Hg Htri.
-          assert (tri = (r, (l, w), r')) by set_solver; subst.
-          contradiction Hr'.
+          assert (tri = (root, rdiff, newroot)) by set_solver; subst.
+          contradiction Hnewroot.
           eapply right_vertex; eauto. }
         set_solver.
       }
     - (* coherent *)
       destruct Hcoh as [X1 X2].
-      constructor.
-      { intros r0 ?. destruct_decide (decide (r0=r')).
+      { constructor.
+      - intros l ?. destruct_decide (decide (l=newroot)).
         { subst. rewrite lookup_insert. inversion 1. done. }
         rewrite lookup_insert_ne //. intros HM.
-        apply X1 in HM. rewrite dom_insert_lookup_L //. }
-      { intros ?. set_solver. }
+        apply X1 in HM. rewrite dom_insert_lookup_L //.
+      - intros ?. set_solver.
+      - set_solver.
+      }
     - (* rooted_dag *)
       eauto using rooted_dag_add.
     - (* global_gen_inv *)
-      assert (not (captured C r')) as Hncapr'.
+      assert (not (captured C newroot)) as CAPnr.
       {
-        intros (σ' & r'gen & Hr'C).
-        assert (r' ∈ dom M) as Hr'M.
+        intros (σ' & nrgen & HnrC).
+        assert (newroot ∈ dom M) as HnrM.
         {
           rewrite elem_of_dom.
           unfold snapshots_inv, snapshot_inv in Hsnap.
-          destruct (Hsnap r' σ' r'gen Hr'C) as (σ'', (H', _)).
+          destruct (Hsnap newroot σ' nrgen HnrC) as (σ'', (H', _)).
           eexists; eauto.
         }
         destruct Hinv.
-        erewrite -> si1M0 in Hr'M.
+        erewrite -> si1M0 in HnrM.
         set_solver.
       }
       { constructor.
@@ -1657,16 +1756,15 @@ Section pstore_G.
           rewrite lookup_insert_ne; first eauto.
           destruct Hglobgen as [Hglobgen1 Hglobgen2].
           unfold gen_succ_rel in Hglobgen2.
-          destruct (G !! r) as [ gr | ] eqn:Hgr; last contradiction Hglobgen2.
-          rewrite Hgr.
-          apply Hglobgen2.
-        - assert (forall n, n ∈ vertices h -> r' ≠ n) as Hnotr'.
+          destruct (G !! root) as [ groot | ] eqn:Hgroot;
+            rewrite Hgroot; rewrite Hgroot in Hglobgen2; apply Hglobgen2.
+        - assert (forall n, n ∈ vertices h -> newroot ≠ n) as Hnotnr.
           {
             intros n Hn Heq; subst n.
-            rewrite -(history_vertices g r h orig) in Hn; eauto.
+            rewrite -(history_vertices g root h orig) in Hn; eauto.
           }
-          rewrite lookup_insert_ne; first (apply Hnotr'; eauto; eapply right_vertex; eauto).
-          rewrite lookup_insert_ne in Hgk; first (apply Hnotr'; eauto; eapply left_vertex; eauto).
+          rewrite lookup_insert_ne; first (apply Hnotnr; eauto; eapply right_vertex; eauto).
+          rewrite lookup_insert_ne in Hgk; first (apply Hnotnr; eauto; eapply left_vertex; eauto).
           destruct Hglobgen as [Hglobgen1 Hglobgen2].
           apply (Hglobgen1 k gk j); eauto.
           eexists; eauto.
@@ -1674,8 +1772,8 @@ Section pstore_G.
       - (* gen_succ_rel between the store generation and the current root *)
         unfold gen_succ_rel.
         rewrite lookup_insert.
-        { destruct_decide (decide (captured C r')).
-        - by contradiction Hncapr'.
+        { destruct_decide (decide (captured C newroot)).
+        - by contradiction CAPnr.
         - trivial. }
       }
     - (* snapshots *)
@@ -1683,10 +1781,10 @@ Section pstore_G.
       iPureIntro.
       intros r0 ? ? HC. apply Hsnap in HC.
       unfold snapshot_inv. destruct HC as (?&HC&?&?).
-      assert (r0 ≠ r') as Hneqr0r'.
+      assert (r0 ≠ newroot) as Hneqr0nr.
       { intro Hr0r.
         subst. destruct Hinv as [X1 X2 X3].
-        assert (r' ∉ dom M) as F by set_solver. apply F. by eapply elem_of_dom. }
+        assert (newroot ∉ dom M) as F by set_solver. apply F. by eapply elem_of_dom. }
       rewrite lookup_insert_ne //.
       exists x.
       split_and!; eauto; [].
@@ -1711,124 +1809,128 @@ Section pstore_G.
     wp_load. wp_store. wp_load. iStep 5.
 
     iDestruct "HC" as "[% (%Hsnap & Hmeta & HC)]".
-    iMod (mono_set_insert' (r, σ, gen) with "HC") as "(HC&Hsnap)".
+    iMod (mono_set_insert' (root, σ, gen) with "HC") as "(HC&Hsnap)".
     iModIntro.
     iSplit. 2:iSteps.
 
-    set C' : snapshots_model := {[(r, σ, gen)]} ∪ C.
+    set C' : snapshots_model := {[(root, σ, gen)]} ∪ C.
 
-    assert (gen_succ_rel C' G (1 + gen) r) as HgenC'r. {
+    assert (gen_succ_rel C' G (1 + gen) root) as HgenC'root. {
       destruct Hglobgen as [Hglobgen1 Hglobgen2].
       unfold gen_succ_rel in Hglobgen2.
       unfold gen_succ_rel.
-      destruct (G !! r) as [ rgen | ]; eauto.
-      assert (captured C' r) by (unfold captured; set_solver).
+      destruct (G !! root) as [ rootgen | ] eqn:HGroot; rewrite HGroot; rewrite HGroot in Hglobgen2; eauto.
+      assert (captured C' root) by (unfold captured; set_solver).
       rewrite decide_True; eauto.
-      destruct_decide (decide (captured C r)) as HcapC; lia.
+      destruct_decide (decide (captured C root)) as HcapC; lia.
    }
 
     unfold pstore.
-    iExists t0, r, orig, (1+gen), _, _, _, _, C'.
+    iExists (* r0, root, orig, gen: *) t0, root, orig, (1+gen),
+            (* ρv, ρg: *) _, _,
+            (* g, h: *)   _, _,
+            (* M, C, G: *) _, C', _.
+
     { iSteps; iPureIntro.
 
     - (* topology_inv g M C' *)
       intros l Hl_dom Hl_cap.
-      assert (not (captured C l)) as Hl_cap'
+      assert (not (captured C l)) as CAPl
         by (unfold captured in *; set_solver).
-      apply (Htopo l Hl_dom Hl_cap').
+      apply (Htopo l Hl_dom CAPl).
 
     (* global_gen_inv. *)
     - (* gen_succ_rel between nodes (k, l) *)
       destruct Hglobgen as (Hglobgen1 & Hglobgen2).
       intros k gk l Hkl Hgk.
       unfold gen_succ_rel.
-      pose proof (history_vertices_have_a_generation M C G g r σ σ0 h orig ltac:(eauto) ltac:(eauto))
+      pose proof (history_vertices_have_a_generation M C G g root σ ρv h orig ltac:(eauto) ltac:(eauto))
         as generation_finder.
       destruct (generation_finder l) as (gl & Hgl); first (destruct Hkl; eapply right_vertex; eauto).
       rewrite Hgl.
       pose proof (Hglobgen1 k gk l ltac:(eauto) ltac:(eauto)) as HgenC.
       unfold gen_succ_rel in HgenC.
       rewrite Hgl in HgenC.
-      { destruct_decide (decide (l = r)) as Hlr.
+      { destruct_decide (decide (l = root)) as Hlr.
       - subst l.
-        assert (captured C' r) as HcapC'r by (unfold captured, C'; set_solver).
-        assert (captured C r) as HcapCr.
+        assert (captured C' root) as CAP'root by (unfold captured, C'; set_solver).
+        assert (captured C root) as CAPoot.
         {
-          (* If 'l' is the current root r and has a historic child k (we
-             have (k, r) ∈ h), then the current root must be captured
-             already in C.
+          (* If 'l' is the current root root and has a historic child
+             k (we have (k, root) ∈ h), then the current root must be
+             captured already in C.
 
              The reasoning is a bit subtle:
 
              - if k is on the path from r to orig, then we have the
-               converse relation (r, k) ∈ g, which implies that r is
-               captured by the no_succ invariant: the root has no
-               successor unless it is captured.
+               converse relation (root, k) ∈ g; but the root has no
+               parent unless it is itself captured (no_succ).
 
-             - if k is *not* on path from r to orig, then *some other
-               node* k' is, and we have (k, r) ∈ g and also (k', r) ∈ g,
-               so r must be captured by the at_most_one_child invariant.
+             - if k is *not* on path from root to orig, then *some
+               other node* k' is, and we have (k, root) ∈ g and also
+               (k', root) ∈ g, so the root must be captured by the
+               at_most_one_child invariant.
            *)
           TODO admit.
         }
         rewrite decide_True; eauto.
         rewrite decide_True in HgenC; eauto.
-      - assert (captured C l <-> captured C' l) as Hcapequiv by (unfold captured; set_solver).
-        { destruct_decide (decide (captured C l)) as HcapC; rewrite Hcapequiv in HcapC.
+      - assert (captured C l <-> captured C' l) as CAPequiv by (unfold captured; set_solver).
+        { destruct_decide (decide (captured C l)) as CAPl; rewrite CAPequiv in CAPl.
         - rewrite decide_True; eauto.
         - rewrite decide_False; eauto.
         }
       }
 
     - (* snapshots_inv M C' G *)
-      intros r' ? ? HC. rewrite elem_of_union elem_of_singleton in HC.
+      intros snaproot ? ? HC. rewrite elem_of_union elem_of_singleton in HC.
       { destruct HC as [HC|HC].
       - inversion HC. subst. destruct Hinv.
         destruct Hglobgen as [Hglobgen1 Hglobgen2].
-        exists σ0; split_and!; eauto.
-      - destruct (Hsnap r' σ1 snap_gen) as (σ' & HMr' & Hσ' & Hsnapgen); eauto.
+        exists ρv; split_and!; eauto.
+      - destruct (Hsnap snaproot σ0 snap_gen) as (σ' & HMr' & Hσ' & Hsnapgen); eauto.
         exists σ'; split_and!; eauto.
         unfold gen_succ_rel.
         unfold gen_succ_rel in Hsnapgen.
-        destruct (G !! r') as [ gr' | ]; eauto.
-        assert (captured C r' <-> captured C' r') as Hcapeq. {
-          destruct_decide (decide (r = r')).
-          - subst r.
+        destruct (G !! snaproot) as [ gsnaproot | ]; eauto.
+        assert (captured C snaproot <-> captured C' snaproot) as CAPequiv. {
+          destruct_decide (decide (root = snaproot)).
+          - subst root.
             unfold captured; set_solver.
           - unfold C'.
             unfold captured; set_solver.
         }
-        { destruct_decide (decide (captured C r')) as Hcap; rewrite Hcapeq in Hcap.
+        { destruct_decide (decide (captured C snaproot)) as CAP; rewrite CAPequiv in CAP.
         - rewrite decide_True //.
         - rewrite decide_False //.
         }
     }
   Admitted.
 
-  Definition fsts  (ys:list (location*(location*val)*location)) : list val :=
-    (fun '(x,_,_) => ValLoc x) <$> ys.
+  Definition fsts (ds:list ref_diff_edge) : list val :=
+    (fun '(l,_,_) => ValLoc l) <$> ds.
 
-  Lemma pstore_collect_spec_aux (r r':location) t' (xs:list val) (ys:list (location*(location*val)*location)) (g:graph_store) :
+  Lemma pstore_collect_spec_aux (l root:location) t' (xs:list val) (ds:list ref_diff_edge) (g:graph_store) :
     lst_model' t' xs ->
-    path g r ys r' ->
+    path g l ds root ->
     {{{
-      r' ↦ §Root ∗
-      ([∗ set] '(r, (l, v), r') ∈ g, r ↦ ’Diff{ #(l : location), v, #(r' : location) })
+      root ↦ §Root ∗
+      diff_nodes g
     }}}
-      pstore_collect #r t'
+      pstore_collect #l t'
     {{{ t,
-      RET (#r',t);
-      r' ↦ §Root ∗
-      ([∗ set] '(r, (l, v), r') ∈ g, r ↦ ’Diff{ #(l : location), v, #(r' : location) }) ∗
-      lst_model t (rev_append (fsts ys) xs)
+      RET (#root,t);
+      root ↦ §Root ∗
+      diff_nodes g ∗
+      lst_model t (rev_append (fsts ds) xs)
     }}}.
   Proof.
     iIntros (-> Hpath Φ) "(Hr'&Hg) HΦ".
-    iInduction ys as [|] "IH" forall (r xs r' Hpath); wp_rec.
+    iInduction ds as [|] "IH" forall (l xs root Hpath); wp_rec.
     { inversion Hpath. subst. iSteps. }
     { inversion Hpath. subst.
-      iDestruct (big_sepS_elem_of_acc _ _ (r,b,a2) with "[$]") as "(?&Hg)".
-      { set_solver. } destruct b.
+      iDestruct (big_sepS_elem_of_acc _ _ (l,b,a2) with "[$]") as "(?&Hg)"; eauto.
+      destruct b as (r, (v, refgen)).
       wp_load.
       iSpecialize ("Hg" with "[$]").
       iSpecialize ("IH" with "[%//][$][$][$]").
@@ -1836,18 +1938,18 @@ Section pstore_G.
     }
   Qed.
 
-  Lemma pstore_collect_spec (r r':location) (ys:list (location*(location*val)*location)) (g:graph_store) :
-    path g r ys r' ->
+  Lemma pstore_collect_spec (l root:location) (ds:list ref_diff_edge) (g:graph_store) :
+    path g l ds root ->
     {{{
-      r' ↦ §Root ∗
-      ([∗ set] '(r, (l, v), r') ∈ g, r ↦ ’Diff{ #(l : location), v, #(r' : location) })
+      root ↦ §Root ∗
+      diff_nodes g
     }}}
-      pstore_collect #r §Nil
+      pstore_collect #l §Nil
     {{{ t,
-      RET (#r',t);
-      r' ↦ §Root ∗
-      ([∗ set] '(r, (l, v), r') ∈ g, r ↦ ’Diff{ #(l : location), v, #(r' : location) }) ∗
-      lst_model t (rev (fsts ys))
+      RET (#root,t);
+      root ↦ §Root ∗
+      diff_nodes g ∗
+      lst_model t (rev (fsts ds))
     }}}.
   Proof.
     iIntros (? Φ) "(?&?) HΦ".
@@ -1856,41 +1958,42 @@ Section pstore_G.
     iApply "Go". rewrite -rev_alt //.
   Qed.
 
-  Lemma use_path r g (xs:list (location*(location*val)*location)) r0 x r1 r':
-    list_to_set xs ⊆ g ->
-    path g r (xs ++ [(r0, x, r1)]) r' ->
-    (r0, x, r1) ∈ (list_to_set xs : gset(location*(location*val)*location) ) ->
-    exists ds, path g r0 ds r0 /\ ds ≠ nil.
+  Lemma use_path g j (ds:list ref_diff_edge) k diff l l' :
+    list_to_set ds ⊆ g ->
+    path g j (ds ++ [(k, diff, l)]) l' ->
+    (k, diff, l) ∈ (list_to_set ds : graph_store) ->
+    exists ds', path g k ds' k /\ ds' ≠ nil.
   Proof.
-    revert r r0 r1 r' x. induction xs; intros r r0 r1 r' x ?.
+    revert j k l l' diff. induction ds; intros j k l l' diff ?.
     { set_solver. }
     rewrite -app_comm_cons. inversion 1. subst.
     rewrite list_to_set_cons.
-    destruct_decide (decide ((r0, x, r1) = (r, b, a2))) as X.
-    { inversion X. subst. intros _. clear IHxs.
+    destruct_decide (decide ((k, diff, l) = (j, b, a2))) as X.
+    { inversion X. subst. intros _. clear IHds.
       rewrite app_comm_cons in H0. apply path_snoc_inv in H0.
       destruct H0 as (?&?&?). subst a2.
-      exists (((r, b, r') :: xs)). done. }
-    { intros ?. apply IHxs in H6. 2,3:set_solver.
+      exists (((j, b, l') :: ds)). done. }
+    { intros ?. apply IHds in H6. 2,3:set_solver.
       destruct H6 as (?&?&?). eexists. split; last done.
       eapply path_weak; first done. set_solver. }
   Qed.
 
-  (* [undo xs ys σ] asserts [mirror xs ys] and that [σ = apply_diffl (proj2 <$> ys ++ xs) σ],
+  (* [undo xs ys ρ] asserts [mirror xs ys] and that [σ = apply_diffl (proj2 <$> ys ++ xs) σ],
      ie, ys undo the changes of xs *)
+  (* FIXME: this should be changed to take generations of ρg into account as well. *)
   Inductive undo :
-    list (location*(location*val)*location) -> list (location*(location*val)*location) -> gmap location val -> Prop :=
+    list ref_diff_edge -> list ref_diff_edge -> gmap location val -> Prop :=
   | undo_nil :
     forall σ, undo [] [] σ
   | undo_cons :
-    forall σ r l v v' r' xs ys,
-      σ !! l = Some v' ->
-      undo xs ys (<[l:=v]> σ) ->
-      undo (xs++[(r,(l,v),r')]) ((r',(l,v'),r)::ys) σ.
+    forall σ j r v gen v' gen' k xs ys,
+      σ !! r = Some v' ->
+      undo xs ys (<[r:=v]> σ) ->
+      undo (xs++[(j,(r,(v,gen)),k)]) ((k,(r,(v',gen')),j)::ys) σ.
 
   Lemma use_undo xs ys σ :
     undo xs ys σ ->
-    σ = apply_diffl (proj2 <$> ys ++ xs) σ.
+    σ = apply_diffl (vchange_of_edge <$> ys ++ xs) σ.
   Proof.
     induction 1.
     { done. }
@@ -1906,31 +2009,34 @@ Section pstore_G.
     induction 1; eauto using mirror_cons,mirror_nil.
   Qed.
 
-  Lemma pstore_revert_spec_aux g g1 r t g2 xs r' w σ σ0 :
+  Lemma pstore_revert_spec_aux g g1 j t g2 xs k v0 ρv ρg :
     lst_model' t (fsts (rev xs)) ->
-    locations_of_edges_in g2 (dom σ) ->
+    dom ρv = dom ρg ->
+    references_in g2 (dom ρv) ->
     g2 = list_to_set xs ->
     acyclic g ->
     g2 ⊆ g ->
-    path g r xs r' ->
+    path g j xs k ->
     {{{
-      r' ↦ w ∗
-      ([∗ map] l0↦v0 ∈ σ, l0.[sref_value] ↦ v0) ∗
-      ([∗ set] '(r, (l, v), r') ∈ g1, r ↦ ’Diff{ #(l : location), v, #(r' : location) }) ∗
-      ([∗ set] '(r, (l, v), r') ∈ g2, r ↦ ’Diff{ #(l : location), v, #(r' : location) })
+      k ↦ v0 ∗
+      diff_nodes g1 ∗
+      diff_nodes g2 ∗
+      ref_values ρv ∗
+      ref_generations ρg
     }}}
-      pstore_revert #r' t
+      pstore_revert #k t
     {{{
       RET ();
       ∃ ys,
-      ⌜undo xs ys σ⌝ ∗
-      r ↦ §Root ∗
-      ([∗ set] '(r, (l, v), r') ∈ (g1 ∪ list_to_set ys), r ↦ ’Diff{ #(l : location), v, #(r' : location) }) ∗
-      ([∗ map] l0↦v0 ∈ (apply_diffl (proj2 <$> xs) σ), l0.[sref_value] ↦ v0)
+      ⌜undo xs ys ρv⌝ ∗
+      j ↦ §Root ∗
+      diff_nodes (g1 ∪ list_to_set ys) ∗
+      ref_values (apply_diffl (vchange_of_edge <$> xs) ρv) ∗
+      ref_generations (apply_diffl (gchange_of_edge <$> xs) ρg)
     }}}.
   Proof.
-    iIntros (-> Hlocs Hg Hacy Hsub Hpath Φ) "(Hr'&Hσ&Hg1&Hg2) HΦ".
-    iInduction xs as [|((r0,(l,v)),r1) ] "IH" using rev_ind forall (σ w r r' g1 g2  Hpath Hg Hlocs Hacy Hsub).
+    iIntros (-> Hdoms Hlocs Hg Hacy Hsub Hpath Φ) "(Hv & Hg1 & Hg2 & Hρv & Hρg) HΦ".
+    iInduction xs as [ | ((l,(r,diff)),l') ] "IH" using rev_ind forall (ρv ρg Hdoms v0 j k g1 g2 Hpath Hg Hlocs Hacy Hsub).
     { wp_rec. simpl.
       iStep 4. iModIntro.
       inversion Hpath. subst. wp_store. iModIntro.
@@ -1940,73 +2046,83 @@ Section pstore_G.
       iStep 4. iModIntro.
       rewrite Hg list_to_set_app_L list_to_set_cons list_to_set_nil right_id_L.
       rewrite Hg list_to_set_app_L in Hsub.
-      assert ((r0, (l, v), r1) ∉ (list_to_set xs : gset (location * diff * location))).
+      assert ((l, (r, (diff : reference_model)), l') ∉ (list_to_set xs : gset ref_diff_edge)).
       { intros ?. apply use_path in Hpath; last done.
         - destruct Hpath as (?&Hpath&?).
           apply Hacy in Hpath. congruence.
         - set_solver. }
-      iDestruct (big_sepS_union with "Hg2") as "(Hg2&?)".
+      iDestruct (big_sepS_union with "Hg2") as "(Hg2&Hldiff)".
       { set_solver. }
+      destruct diff as (refv, refgen).
       rewrite big_sepS_singleton. wp_load. iStep 4. iModIntro.
 
       rewrite Hg list_to_set_app_L list_to_set_cons list_to_set_nil right_id_L in Hlocs.
-      assert (exists v', σ !! l = Some v') as (v',Hl).
+      assert (exists v, ρv !! r = Some v) as (v,Hv).
       { apply elem_of_dom. eapply Hlocs. rewrite /edge.
-
         rewrite elem_of_union elem_of_singleton. right. reflexivity. }
+
+      assert (exists gen, ρg !! r = Some gen) as (gen, Hgen).
+      { apply (use_r_in_dom ρv ρg r v); set_solver. }
 
       apply path_snoc_inv in Hpath. destruct Hpath as (?&->&?).
       wp_smart_apply assert_spec. { rewrite bool_decide_eq_true_2 //. }
       iStep 4. iModIntro.
 
-      iDestruct (big_sepM_insert_acc with "Hσ") as "(Hl & Hσ)"; first done.
+      iDestruct (big_sepM_insert_acc with "Hρv") as "(Hrv & Hρv)"; first done.
+      iDestruct (big_sepM_insert_acc with "Hρg") as "(Hrg & Hρg)"; first done.
 
-      wp_load. wp_store. wp_store. iStep 4. iModIntro.
+      wp_load. wp_load. wp_store. wp_store. wp_store. iStep 4. iModIntro.
 
-      iSpecialize ("Hσ" with "[$]").
-      iSpecialize ("IH" with "[%//][%//][%][%//][%][$][$] Hg1 Hg2").
-      { rewrite dom_insert_lookup_L //. intros x1 x2 x3 x4.
-        specialize (Hlocs x1 x2 x3 x4). set_solver. }
+      iSpecialize ("Hρv" with "[$]").
+      iSpecialize ("Hρg" with "[$]").
+      iSpecialize ("IH" $! (<[r:=refv]> ρv) (<[r:=refgen]> ρg) with "[%][%//][%//][%][%//][%][$] Hg1 Hg2 [$][$]").
+      { do 2 rewrite dom_insert_L. set_solver. }
+      { rewrite dom_insert_L. intros j' r' w' l'.
+        specialize (Hlocs j' r' w' l'). set_solver. }
       { set_solver. }
 
-      rewrite fmap_app -apply_diffl_snoc. simpl.
+      do 2 rewrite fmap_app -apply_diffl_snoc. simpl.
       iApply "IH". iModIntro.
-      iIntros "[%ys (%Hundo&?&?&?)]". iApply "HΦ".
-      iExists ((r',(l,v'),r0)::ys). iFrame.
+      iIntros "[%ys (%Hundo&?&?&?&?)]". iApply "HΦ".
+      iExists ((k,(r,(v,gen)),l)::ys). iFrame.
       iSplitR.
       { iPureIntro. eauto using undo_cons. }
       rewrite list_to_set_cons.
-      iAssert ⌜(r', (l, v'), r0) ∉ g1 ∪ list_to_set ys⌝%I as "%".
+      iAssert ⌜(k, (r, (v,gen)), l) ∉ g1 ∪ list_to_set ys⌝%I as "%".
       { iIntros (?). iDestruct (big_sepS_elem_of with "[$]") as "?"; first done.
-        iDestruct (pointsto_ne r' r' with "[$][$]") as "%". congruence. }
-      replace (g1 ∪ ({[(r', (l, v'), r0)]} ∪ list_to_set ys)) with ({[(r', (l, v'), r0)]} ∪ ((g1 ∪ list_to_set ys))). 2:set_solver.
-      iApply big_sepS_union; first set_solver.
-      iFrame. rewrite big_sepS_singleton //. }
+        iDestruct (pointsto_ne k k with "[$][$]") as "%". congruence. }
+      replace (g1 ∪ ({[(k, (r, (v, gen)), l)]} ∪ list_to_set ys)) with ({[(k, (r, (v, gen)), l)]} ∪ ((g1 ∪ list_to_set ys))); last set_solver.
+      iApply big_sepS_union ; first set_solver.
+      iFrame. rewrite big_sepS_singleton //.
+    }
   Qed.
 
-  Lemma pstore_revert_spec r t g xs r' w σ σ0 :
+  Lemma pstore_revert_spec j t g xs k v0 ρv ρg :
     lst_model' t (fsts (rev xs)) ->
-    locations_of_edges_in g (dom σ) ->
+    dom ρv = dom ρg ->
+    references_in g (dom ρv) ->
     g = list_to_set xs ->
     acyclic g ->
-    path g r xs r' ->
+    path g j xs k ->
     {{{
-      r' ↦ w ∗
-      ([∗ map] l0↦v0 ∈ σ, l0.[sref_value] ↦ v0) ∗
-      ([∗ set] '(r, (l, v), r') ∈ g, r ↦ ’Diff{ #(l : location), v, #(r' : location) })
+      k ↦ v0 ∗
+      diff_nodes g ∗
+      ref_values ρv ∗
+      ref_generations ρg
     }}}
-      pstore_revert #r' t
+      pstore_revert #k t
     {{{
       RET ();
       ∃ ys,
-      ⌜undo xs ys σ⌝ ∗
-      r ↦ §Root ∗
-      ([∗ set] '(r, (l, v), r') ∈ (list_to_set ys), r ↦ ’Diff{ #(l : location), v, #(r' : location) }) ∗
-      ([∗ map] l0↦v0 ∈ (apply_diffl (proj2 <$> xs) σ), l0.[sref_value] ↦ v0)
+      ⌜undo xs ys ρv⌝ ∗
+      j ↦ §Root ∗
+      diff_nodes (list_to_set ys) ∗
+      ref_values (apply_diffl (vchange_of_edge <$> xs) ρv) ∗
+      ref_generations (apply_diffl (gchange_of_edge <$> xs) ρg)
     }}}.
   Proof.
-    iIntros (->???? Φ) "(?&?&?) HΦ".
-    iApply (pstore_revert_spec_aux g ∅ with "[-HΦ]"); try done.
+    iIntros (Hxs Hdom Hgrefs Dg Hacy Pxs Φ) "(Hk & Hnodes & Hρv & Hρg) HΦ".
+    iApply (pstore_revert_spec_aux g ∅ j t g xs k v0 ρv ρg Hxs Hdom Hgrefs Dg Hacy ltac:(set_solver) Pxs with "[-HΦ]"); try done.
     { rewrite big_sepS_empty. iFrame. }
     { iModIntro. iIntros "[% ?]". iApply "HΦ". iExists _. rewrite left_id_L //. }
   Qed.
@@ -2018,52 +2134,69 @@ Section pstore_G.
     rewrite IHxs /fsts fmap_app //.
   Qed.
 
-  Lemma pstore_reroot_spec r (xs:list (location*(location*val)*location)) r' g σ :
-    locations_of_edges_in g (dom σ) ->
+  Lemma pstore_reroot_spec j (xs:list ref_diff_edge) k g ρv ρg :
+    references_in g (dom ρv) ->
+    dom ρv = dom ρg ->
     g = list_to_set xs ->
     acyclic g ->
-    path g r xs r' ->
+    path g j xs k ->
     {{{
-      r' ↦ §Root ∗
-      ([∗ map] l0↦v0 ∈ σ, l0.[sref_value] ↦ v0) ∗
-      ([∗ set] '(r, (l, v), r') ∈ g, r ↦ ’Diff{ #(l : location), v, #(r' : location) })
+      k ↦ §Root ∗
+      diff_nodes g ∗
+      ref_values ρv ∗
+      ref_generations ρg
     }}}
-      pstore_reroot #r
+      pstore_reroot #j
     {{{
       RET ();
       ∃ ys,
-      ⌜undo xs ys σ⌝ ∗
-      r ↦ §Root ∗
-      ([∗ set] '(r, (l, v), r') ∈ (list_to_set ys), r ↦ ’Diff{ #(l : location), v, #(r' : location) }) ∗
-      ([∗ map] l0↦v0 ∈ (apply_diffl (proj2 <$> xs) σ), l0.[sref_value] ↦ v0)
+      ⌜undo xs ys ρv⌝ ∗
+      j ↦ §Root ∗
+      diff_nodes (list_to_set ys) ∗
+      ref_values (apply_diffl (vchange_of_edge <$> xs) ρv) ∗
+      ref_generations (apply_diffl (gchange_of_edge <$> xs) ρg)
     }}}.
   Proof.
-    iIntros (???? Φ) "(Hr'&Hσ&Hg) HΦ".
+    iIntros (Hgdom Hdoms Dg Hacy Pxs Φ) "(Hk & Hnodes & Hρv & Hρg) HΦ".
     wp_rec. wp_apply (pstore_collect_spec with "[$]"); first done.
-    iIntros (?) "(?&?&%Heq)". rewrite {}Heq.
+    iIntros (t) "(Hk & Hnodes & %Ht)". rewrite {}Ht.
     wp_smart_apply (pstore_revert_spec with "[-HΦ]"); try done; first rewrite rev_fsts //.
     iSteps.
   Qed.
 
-  Lemma locations_of_edges_weak g1 g2 X :
-    locations_of_edges_in g1 X ->
+  Lemma references_in_weak g1 g2 X :
+    references_in g1 X ->
     g2 ⊆ g1 ->
-    locations_of_edges_in g2 X.
+    references_in g2 X.
   Proof.
     intros Z ? a b c d ?. eapply (Z a b c d). set_solver.
   Qed.
 
-  Lemma undo_same_fst_label xs ys r l v r' σ :
+  Lemma undo_same_fst_label xs ys j r w k σ :
     undo xs ys σ ->
-    (r, (l, v), r') ∈ (list_to_set ys :  gset (location*(location*val)*location)) ->
-    l ∈ (list_to_set (proj2 <$> xs).*1 : gset location).
+    (j, (r, w), k) ∈ (list_to_set ys : gset ref_diff_edge) ->
+    r ∈ (list_to_set (proj2 <$> xs).*1 : gset ref_loc).
   Proof.
     revert xs σ. induction ys as [|(?,?)]; first set_solver.
     intros xs σ. inversion 1. subst.
     simpl. rewrite !fmap_app list_to_set_app_L. simpl in *. subst.
-    destruct_decide (decide ((r, (l, v), r') = (r'0, (l1, v'), l0))) as Heq.
+    destruct_decide (decide ((j, (r, w), k) = (k0, (r0, (v', gen')), n))) as Heq.
     { inversion Heq. subst. intros _. set_solver. }
     intros ?. simpl. apply elem_of_union. left. eapply IHys; first done. set_solver.
+  Qed.
+
+  Lemma vchange_fst_label (ds : list ref_diff_edge) :
+    (proj2 <$> ds).*1 = (vchange_of_edge <$> ds).*1.
+  Proof.
+    induction ds as [ | ((j, (r, (v, refgen))), k) ds ]; eauto.
+    - cbn. by rewrite IHds.
+  Qed.
+
+  Lemma gchange_fst_label (ds : list ref_diff_edge) :
+    (proj2 <$> ds).*1 = (gchange_of_edge <$> ds).*1.
+  Proof.
+    induction ds as [ | ((j, (r, (v, refgen))), k) ds ]; eauto.
+    - cbn. by rewrite IHds.
   Qed.
 
   Definition diff_last {A:Type} (ys1 ys2:list A) :=
@@ -2074,16 +2207,16 @@ Section pstore_G.
         True
     end.
 
-  Lemma path_extract_suffix (g:gset (location*(location*val)*location)) a1 a2 xs1 r xs2 :
+  Lemma path_extract_suffix (g:gset ref_diff_edge) a1 a2 xs1 root xs2 :
     unaliased g ->
-    path g a1 xs1 r ->
-    path g a2 xs2 r  ->
+    path g a1 xs1 root ->
+    path g a2 xs2 root  ->
     exists ys1 ys2 xs,
       xs1 = ys1 ++ xs /\
       xs2 = ys2 ++ xs /\ diff_last ys1 ys2.
   Proof.
     intros Hinj.
-    revert r a1 a2 xs2. induction xs1 using rev_ind; intros r a1 a2 xs2.
+    revert root a1 a2 xs2. induction xs1 using rev_ind; intros root a1 a2 xs2.
     { inversion 1. subst. intros. exists nil,xs2,nil.
       simpl. rewrite right_id_L. set_solver. }
     intros Hp1 Hp2. apply path_inv_r in Hp1.
@@ -2092,8 +2225,8 @@ Section pstore_G.
     apply app_inj_tail in X1. destruct X1 as (<-&->).
 
     apply path_inv_r in Hp2. destruct Hp2 as [(->&->) | (bs'&b&y'&->&?&?)].
-    { exists (xs1 ++ [(y, b', r)]),nil,nil. rewrite right_id. split_and !; try done.
-      unfold diff_last. destruct (last (xs1 ++ [(y, b', r)])); try done. }
+    { exists (xs1 ++ [(y, b', root)]),nil,nil. rewrite right_id. split_and !; try done.
+      unfold diff_last. destruct (last (xs1 ++ [(y, b', root)])); try done. }
 
     destruct_decide (decide (y'=y)); last first.
     { eexists _,_,nil. rewrite !right_id_L. split_and!; try done.
@@ -2102,7 +2235,7 @@ Section pstore_G.
 
     destruct (IHxs1 _ _ _ _ X2 H) as (ys1&ys2&xs&->&->&Hdiff).
     destruct (Hinj _ _ _ _ _ X3 H0) as (->&_).
-    eexists _,_,(xs++[(y, b, r)]). rewrite !assoc_L. done.
+    eexists _,_,(xs++[(y, b, root)]). rewrite !assoc_L. done.
   Qed.
 
   Lemma diff_last_app_middle {A:Type} x (l1' l2' l1 l2:list A) :
@@ -2122,11 +2255,11 @@ Section pstore_G.
     rewrite !last_app //. simpl. naive_solver.
   Qed.
 
-  Lemma path_use_diff_last (g:gset (location*(location*val)*location)) a1 a2 ys1 ys2 xs r :
+  Lemma path_use_diff_last (g:gset ref_diff_edge) a1 a2 ys1 ys2 xs root :
     acyclic g ->
     unaliased g ->
-    path g a1 (ys1 ++ xs) r ->
-    path g a2 (ys2 ++ xs) r  ->
+    path g a1 (ys1 ++ xs) root ->
+    path g a2 (ys2 ++ xs) root  ->
     diff_last ys1 ys2 ->
     forall x, x ∈ ys2 -> x ∉ (ys1 ++ xs).
   Proof.
@@ -2172,11 +2305,11 @@ Section pstore_G.
   Qed.
 
   Lemma path_use_diff_last_subseteq
-    g (a1 a2 : location) (ys1 ys2 xs : list (location * diff * location)) (r : location) :
+    g (a1 a2 : node_loc) (ys1 ys2 xs : list ref_diff_edge) (root : node_loc) :
     acyclic g ->
     unaliased g ->
-    path g a1 (ys1 ++ xs) r ->
-    path g a2 (ys2 ++ xs) r ->
+    path g a1 (ys1 ++ xs) root ->
+    path g a2 (ys2 ++ xs) root ->
     diff_last ys1 ys2 ->
     list_to_set ys2 ⊆ g ∖ list_to_set (ys1 ++ xs).
   Proof.
@@ -2187,7 +2320,7 @@ Section pstore_G.
       rewrite elem_of_list_to_set in Hel2.
       eapply (path_use_diff_last g a1 a2); eauto.
     -
-      destruct (path_middle g a2 ys2 xs r ltac:(subst; auto))
+      destruct (path_middle g a2 ys2 xs root ltac:(subst; auto))
         as (mid & Hmid1 & Hmid2).
       eapply path_all_in; eauto.
   Qed.
@@ -2199,7 +2332,7 @@ Section pstore_G.
     destruct (last l1),(last l2); naive_solver.
   Qed.
 
-  Lemma path_union_inv (g1: graph location (location*val)) g2 a1 xs a2 :
+  Lemma path_union_inv (g1: graph_store) g2 a1 xs a2 :
     path (g1 ∪ g2) a1 xs a2 ->
     path g1 a1 xs a2 \/ exists a' x xs1 xs2, path g1 a1 xs1 a' /\ x ∈ g2 /\ path (g1 ∪ g2) a' (x::xs2) a2 /\ xs=xs1++x::xs2.
   Proof.
@@ -2228,11 +2361,11 @@ Section pstore_G.
     }
   Qed.
 
-  Lemma path_cannot_escape (x:(location * diff * location)) (xs ys:list (location * diff * location)) (g1: graph location (location*val)) a a' r :
-    no_succ (g1 ∪ list_to_set ys) r ->
+  Lemma path_cannot_escape (x: ref_diff_edge) (xs ys:list ref_diff_edge) (g1: graph_store) a a' root :
+    no_succ (g1 ∪ list_to_set ys) root ->
     unaliased (g1 ∪ list_to_set ys) ->
     x ∈ (list_to_set ys : gset _) ->
-    pathlike ys r ->
+    pathlike ys root ->
     path (g1 ∪ list_to_set ys) a (x :: xs) a' ->
     path (list_to_set ys) a (x::xs) a'.
   Proof.
@@ -2245,16 +2378,16 @@ Section pstore_G.
     eapply IHzs; eauto. inversion H6. subst.
     apply elem_of_list_to_set in X2. apply X3 in X2.
     { destruct X2 as [|(?&?&?)].
-    - subst. contradiction H with l0. eexists. eauto.
-    - assert ((l, x, x0) ∈  g1 ∪ list_to_set ys) as Z by set_solver.
+    - subst. contradiction H with n0. eexists. eauto.
+    - assert ((n, x, x0) ∈  g1 ∪ list_to_set ys) as Z by set_solver.
       destruct (X1 _ _ _ _ _ H9 Z). subst. set_solver.
     }
   Qed.
 
-  Lemma path_in_seg_complete (r a a':location) (x:(location * diff * location)) (xs0 xs1 ys: list (location * diff * location)) (g1:graph location (location*val)) :
-    no_succ (g1 ∪ list_to_set ys) r ->
+  Lemma path_in_seg_complete (root a a':node_loc) (x:ref_diff_edge) (xs0 xs1 ys: list ref_diff_edge) (g1:graph_store) :
+    no_succ (g1 ∪ list_to_set ys) root ->
     unaliased (g1 ∪ list_to_set ys) ->
-    pathlike ys r ->
+    pathlike ys root ->
     path (g1 ∪ list_to_set ys) a xs0 a' ->
     path (list_to_set ys) a' (x :: xs1) a ->
     exists zs, path (list_to_set ys) a zs a'.
@@ -2273,14 +2406,14 @@ Section pstore_G.
     destruct (Hinj _ _ _ _ _ H Z). set_solver.
   Qed.
 
-  Lemma undo_preserves_rooted_dag (g:graph location (location*val)) xs ys rs r :
-    no_succ (undo_graph g xs ys) rs ->
+  Lemma undo_preserves_rooted_dag (g:graph_store) xs ys snaproot root :
+    no_succ (undo_graph g xs ys) snaproot ->
     unaliased g ->
     unaliased (list_to_set ys ∪ g ∖ list_to_set xs) ->
-    path g rs xs r ->
+    path g snaproot xs root ->
     mirror xs ys ->
-    rooted_dag g r ->
-    rooted_dag (undo_graph g xs ys) rs.
+    rooted_dag g root ->
+    rooted_dag (undo_graph g xs ys) snaproot.
   Proof.
     intros Hnr Hinj Hinj' Hpath Hmirror Hroot. inversion Hroot as [X1 X2].
     assert (vertices (undo_graph g xs ys) = vertices g) as Hvg.
@@ -2291,7 +2424,7 @@ Section pstore_G.
     constructor.
     { intros a. rewrite Hvg => Ha.
       apply X1 in Ha. destruct Ha as (zs&Ha).
-      edestruct (path_extract_suffix g a rs) as (ys1&ys2&us&?&?&Hlast); eauto. subst.
+      edestruct (path_extract_suffix g a snaproot) as (ys1&ys2&us&?&?&Hlast); eauto. subst.
 
       apply path_middle in Ha. destruct Ha as (y&Hy1&Hy2).
       apply path_middle in Hpath. destruct Hpath as (y'&Hy'1&Hy'2).
@@ -2322,14 +2455,14 @@ Section pstore_G.
          We are going to construct a cycle in ys, implying a cycle in xs. *)
       exfalso. destruct Hsz as (a'&x&l1&l2&E1&Hx&E2&->).
 
-      apply path_cannot_escape with (r:=rs) in E2; last first.
+      apply path_cannot_escape with (root:=snaproot) in E2; last first.
       { eapply path_pathlike. eapply use_mirror; eauto. }
       { done. }
       { rewrite comm_L //. }
       { rewrite comm_L //. }
 
       apply path_weak with (g2 := g ∖ list_to_set xs ∪ list_to_set ys) in E1; last set_solver.
-      eapply path_in_seg_complete with (r:=rs) in E1; last first; first done.
+      eapply path_in_seg_complete with (root:=snaproot) in E1; last first; first done.
       { eapply path_pathlike. eapply use_mirror; eauto. }
       { rewrite comm_L //. }
       { rewrite comm_L //. }
@@ -2348,7 +2481,7 @@ Section pstore_G.
 
   Lemma undo_app_inv xs ys1 ys2 σ :
     undo xs (ys1 ++ ys2) σ ->
-    exists xs1 xs2, xs = xs2 ++ xs1 /\ undo xs2 ys2 (apply_diffl (proj2 <$> xs1) σ) /\ undo xs1 ys1 σ.
+    exists xs1 xs2, xs = xs2 ++ xs1 /\ undo xs2 ys2 (apply_diffl (vchange_of_edge <$> xs1) σ) /\ undo xs1 ys1 σ.
   Proof.
     revert xs ys2 σ. induction ys1; intros xs ys2 σ Hundo.
     { exists nil,xs. rewrite right_id_L. split; eauto using undo_nil. }
@@ -2360,7 +2493,7 @@ Section pstore_G.
     { apply undo_cons; done. }
   Qed.
 
-  Lemma construct_middlepoint (g:graph location (location*val)) a1 xs ys a2 a2' :
+  Lemma construct_middlepoint g a1 xs ys a2 a2' :
     unaliased g ->
     no_succ g a2 ->
     path g a1 xs a2 ->
@@ -2377,17 +2510,17 @@ Section pstore_G.
     }
   Qed.
 
-  Lemma undo_preserves_model g (M:map_model) (xs ys:list (location* (location*val)*location)) rs σ0 r:
-    dom M = vertices g ∪ {[r]} ->
+  Lemma undo_preserves_model g (M:map_model) (xs ys:list ref_diff_edge) snaproot ρ root :
+    dom M = vertices g ∪ {[root]} ->
     correct_path_diff M g ->
-    no_succ (undo_graph g xs ys) rs ->
+    no_succ (undo_graph g xs ys) snaproot ->
     unaliased (undo_graph g xs ys) ->
-    path g rs xs r ->
-    undo xs ys σ0 ->
-    M !! r = Some σ0 ->
+    path g snaproot xs root ->
+    undo xs ys ρ ->
+    M !! root = Some ρ ->
     correct_path_diff M (undo_graph g xs ys).
   Proof.
-    intros Hdom Hinv Hroot Hinj' Hrs Hundo E0.
+    intros Hdom Hinv Hroot Hinj' Hsnaproot Hundo E0.
     unfold undo_graph.
     intros r1 zs r2 σ1 σ2 Hpath E1 E2. rewrite comm_L in Hpath.
     apply path_union_inv in Hpath. destruct Hpath as [Hpath|Hpath].
@@ -2398,7 +2531,7 @@ Section pstore_G.
     assert (mirror xs ys) as Hmirror by eauto using undo_mirror.
 
     destruct Hpath as (a'&x&l1&l2&X1&Hx&X2&Hzs).
-    eapply path_cannot_escape with (r:=rs) in X2; eauto; last first.
+    eapply path_cannot_escape with (root:=snaproot) in X2; eauto; last first.
     { eapply path_pathlike. eapply use_mirror; eauto. }
     { replace (g ∖ list_to_set xs ∪ list_to_set ys)
                 with (undo_graph g xs ys) by set_solver.
@@ -2416,7 +2549,7 @@ Section pstore_G.
     { rewrite Hdom -Hvg elem_of_union. left. apply elem_of_vertices.
       inversion X2. set_solver. }
     apply elem_of_dom in Ha'. destruct Ha' as (σ',Ea').
-    assert (σ1 = (apply_diffl (proj2 <$> l1) σ')).
+    assert (σ1 = (apply_diffl (vchange_of_edge <$> l1) σ')).
     { eapply path_weak in X1.
     - eapply (Hinv _ _ _ _ _ X1 E1 Ea').
     - set_solver.
@@ -2428,10 +2561,10 @@ Section pstore_G.
 
     (* XXX facto a lemma. *)
     assert (exists u1 u2, ys = u1 ++ (x::l2) ++ u2) as (u1&u2&Hys).
-    { eapply use_mirror in Hrs. 2:done.
+    { eapply use_mirror in Hsnaproot. 2:done.
       apply elem_of_list_to_set, elem_of_middle in Hx.
       destruct Hx as (p1&p2&->).
-      apply path_app_inv in Hrs. destruct Hrs as (?&Hp1&Hp2).
+      apply path_app_inv in Hsnaproot. destruct Hsnaproot as (?&Hp1&Hp2).
       inversion Hp2; inversion X2. subst. inversion H5. subst.
       eapply construct_middlepoint in H10. 4:apply H4.
       2:{ unfold undo_graph in *.
@@ -2456,16 +2589,16 @@ Section pstore_G.
     edestruct (same_path (list_to_set ys) (x::l2) n1 n2 a') as (?&?); try done.
     subst n1 n2.
 
-    assert (path g a' xs4 r) as R1.
+    assert (path g a' xs4 root) as R1.
     { eapply path_weak.
     - eapply use_mirror; last done. eapply mirror_symm. eauto using undo_mirror.
-    - apply path_all_in in Hrs. set_solver. }
-    apply (Hinv _ _ _ σ' σ0) in R1; try done.
+    - apply path_all_in in Hsnaproot. set_solver. }
+    apply (Hinv _ _ _ σ' ρ) in R1; try done.
 
     assert (path g r2 xs3 a') as R2.
     { eapply path_weak.
     - eapply use_mirror; last done. eapply mirror_symm. eauto using undo_mirror.
-    - apply path_all_in in Hrs. set_solver. }
+    - apply path_all_in in Hsnaproot. set_solver. }
     eapply (Hinv _ _ _ σ2 σ') in R2; try done.
     rewrite R2. rewrite -apply_diffl_app -fmap_app.
     eapply use_undo. rewrite R1. done.
@@ -2515,16 +2648,16 @@ Section pstore_G.
    }
   Qed.
 
-  Lemma into_a_path g rs xs r :
+  Lemma into_a_path g snaproot xs root :
     unaliased g ->
-    path g rs xs r ->
+    path g snaproot xs root ->
     forall k1 d1 k d2 k2,
     edge (g ∖ list_to_set xs) k1 d1 k ->
     edge (list_to_set xs) k d2 k2 ->
-    k = rs \/ (exists k1' d1', k1 ≠ k1' /\ edge (list_to_set xs) k1' d1' k)
+    k = snaproot \/ (exists k1' d1', k1 ≠ k1' /\ edge (list_to_set xs) k1' d1' k)
   .
   Proof.
-    { revert rs. induction xs; intro rs.
+    { revert snaproot. induction xs; intro snaproot.
     - set_solver.
     - rewrite list_to_set_cons.
       unfold edge.
@@ -2544,10 +2677,10 @@ Section pstore_G.
           constructor; first assumption.
           intro hyp. apply H1xs. right. assumption.
         - replace a2 with k in *.
-          right. exists rs, b.
+          right. exists snaproot, b.
           { constructor.
           - intro Heq. apply H1xs. left.
-            subst. destruct (Hunaliased rs d1 k b k); auto.
+            subst. destruct (Hunaliased snaproot d1 k b k); auto.
             subst. reflexivity.
           - set_solver. }
         - right.
@@ -2557,19 +2690,19 @@ Section pstore_G.
     }
   Qed.
 
-  Lemma into_a_path_captured g C M rs xs r :
-    dom M = vertices g ∪ {[r]} ->
-    topology_inv g M C r ->
+  Lemma into_a_path_captured g C M snaproot xs root :
+    dom M = vertices g ∪ {[root]} ->
+    topology_inv g M C root ->
     unaliased g ->
-    captured C rs ->
-    path g rs xs r ->
+    captured C snaproot ->
+    path g snaproot xs root ->
     forall k1 d1 k d2 k2,
     edge (g ∖ list_to_set xs) k1 d1 k ->
     edge (list_to_set xs) k d2 k2 ->
     not (not (captured C k))
   .
     intros Hdom Htopo Hunaliased Hcap Hpath k1 d1 k d2 k2 Hk1 Hk2 Hk_cap.
-    { destruct (into_a_path g rs xs r Hunaliased Hpath k1 d1 k d2 k2) as [ Hend | Hmid ]; eauto.
+    { destruct (into_a_path g snaproot xs root Hunaliased Hpath k1 d1 k d2 k2) as [ Hend | Hmid ]; eauto.
     - subst. exact (Hk_cap Hcap).
     - destruct Hmid as (k1' & d1' & Hneq & Hedge).
       assert (k ∈ dom M).
@@ -2589,43 +2722,43 @@ Section pstore_G.
     }
   Qed.
 
-  Lemma undo_preserves_topo g M C (xs ys:list (location* (location*val)*location)) r rs :
-    dom M = vertices g ∪ {[r]} ->
+  Lemma undo_preserves_topo g M C (xs ys:list ref_diff_edge) root snaproot :
+    dom M = vertices g ∪ {[root]} ->
     unaliased g ->
-    captured C rs ->
-    path g rs xs r ->
+    captured C snaproot ->
+    path g snaproot xs root ->
     mirror xs ys ->
-    topology_inv g M C r ->
-    topology_inv (undo_graph g xs ys) M C rs.
+    topology_inv g M C root ->
+    topology_inv (undo_graph g xs ys) M C snaproot.
   Proof.
-    intros Hdom Hunaliased Hrs_cap Hpath Hmirror Htopo.
-    intros k Hk_dom Hk_cap.
+    intros Hdom Hunaliased CAPsnaproot Hpath Hmirror Htopo.
+    intros k Hk_dom CAPk.
     { constructor.
     - intro; subst. contradiction.
     - intros k1 k2 Hk1 Hk2.
-      { destruct (undo_graph_edges g rs xs r ys Hpath Hmirror _ _ Hk1) as [ (d1, Hk1') | (d1, Hk1') ];
-          destruct (undo_graph_edges g rs xs r ys Hpath Hmirror _ _ Hk2) as [ (d2, Hk2') | (d2, Hk2') ];
+      { destruct (undo_graph_edges g snaproot xs root ys Hpath Hmirror _ _ Hk1) as [ (d1, Hk1') | (d1, Hk1') ];
+          destruct (undo_graph_edges g snaproot xs root ys Hpath Hmirror _ _ Hk2) as [ (d2, Hk2') | (d2, Hk2') ];
             clear Hk1 Hk2.
       - { apply (Htopo k); auto.
         - exists d1. set_solver.
         - exists d2. set_solver.
         }
-      - { destruct into_a_path_captured with g C M rs xs r k1 d1 k d2 k2; eauto. }
-      - { destruct into_a_path_captured with g C M rs xs r k2 d2 k d1 k1; eauto. }
+      - { destruct into_a_path_captured with g C M snaproot xs root k1 d1 k d2 k2; eauto. }
+      - { destruct into_a_path_captured with g C M snaproot xs root k2 d2 k d1 k1; eauto. }
       - { eapply Hunaliased; eauto.
-          - apply (path_all_in g rs xs r Hpath); eauto.
-          - apply (path_all_in g rs xs r Hpath); eauto.
+          - apply (path_all_in g snaproot xs root Hpath); eauto.
+          - apply (path_all_in g snaproot xs root Hpath); eauto.
         }
       }
     }
   Qed.
 
-  Lemma undo_preserves_outside_path g r xs rs ys a zs b :
-    path g rs xs r ->
-    path g a zs b ->
+  Lemma undo_preserves_outside_path g root xs snaproot ys j zs k :
+    path g snaproot xs root ->
+    path g j zs k ->
     mirror xs ys ->
     list_to_set zs ⊆ g ∖ list_to_set xs ->
-    path (undo_graph g xs ys) a zs b.
+    path (undo_graph g xs ys) j zs k.
   Proof.
     intros Hxs Hzs Hxsys Hincl.
     apply path_weak with (list_to_set zs); eauto.
@@ -2636,30 +2769,30 @@ Section pstore_G.
       apply Hincl; done.
   Qed.
 
-  Lemma undo_preserves_histo g1 r1 h1 orig r2 xs xsm :
+  Lemma undo_preserves_histo g1 n1 h1 orig n2 xs xsm :
     acyclic g1 ->
     unaliased g1 ->
-    history_inv g1 r1 h1 orig ->
-    path g1 r2 xs r1 ->
+    history_inv g1 n1 h1 orig ->
+    path g1 n2 xs n1 ->
     mirror xs xsm ->
     exists h2,
       graph_iso h1 h2
       /\
-      history_inv (undo_graph g1 xs xsm) r2 h2 orig.
+      history_inv (undo_graph g1 xs xsm) n2 h2 orig.
   Proof.
     intros Hacyclic Hunalias (ys & ysm & Hys & Hysysm & Hhisto) Hxs Hxsxsm.
     unfold history_inv.
     set g2 := undo_graph g1 xs xsm.
     assert (h1 = undo_graph g1 ys ysm) as Hhisto_strict.
     { apply leibniz_equiv; done. }
-    assert (path g2 r1 xsm r2) as Hxsm by (eapply undo_path; eauto).
-    assert (path h1 r1 ysm orig) as Hysm by (subst h1; eapply undo_path; eauto).
+    assert (path g2 n1 xsm n2) as Hxsm by (eapply undo_path; eauto).
+    assert (path h1 n1 ysm orig) as Hysm by (subst h1; eapply undo_path; eauto).
     destruct
-      (path_extract_suffix g1 r2 orig xs r1 ys Hunalias Hxs Hys)
+      (path_extract_suffix g1 n2 orig xs n1 ys Hunalias Hxs Hys)
       as (xs' & ys' & suf & Hxs' & Hys' & Hdiff).
-    destruct (path_middle g1 r2 xs' suf r1 ltac:(subst; auto))
+    destruct (path_middle g1 n2 xs' suf n1 ltac:(subst; auto))
       as (xmid & Hxmid1 & Hxmid2).
-    destruct (path_middle g1 orig ys' suf r1 ltac:(subst; auto))
+    destruct (path_middle g1 orig ys' suf n1 ltac:(subst; auto))
       as (ymid & Hymid1 & Hymid2).
     assert (xmid = ymid) as Hmid; [ | subst ymid ].
     {
@@ -2670,9 +2803,9 @@ Section pstore_G.
     }
     assert (mirror ysm (ys' ++ suf)) as Htemp1 by (subst; apply mirror_symm; done).
     assert (mirror xsm (xs' ++ suf)) as Htemp2 by (subst; apply mirror_symm; done).
-    destruct (mirror_app_inv_in_graph g1 orig ys' xmid suf r1 ysm)
+    destruct (mirror_app_inv_in_graph g1 orig ys' xmid suf n1 ysm)
       as (ys'm & sufm & Dysm & Mys' & Msuf & Psufm & Pys'm); eauto; [].
-    destruct (mirror_app_inv_in_graph g1 r2 xs' xmid suf r1 xsm)
+    destruct (mirror_app_inv_in_graph g1 n2 xs' xmid suf n1 xsm)
       as (xs'm & sufm' & Dysm' & Mxs' & Msuf' & Psufm' & Pxs'm); eauto; [].
 
     (* A bunch of facts that help [set_solver] with the proofs below. *)
@@ -2716,8 +2849,8 @@ Section pstore_G.
          | ys'              ↑ ys'm
          v                  |
        -> \ suf           -> <-
-  xs' /    > r1      xs' /     \ sufm
-     r2                r2       r1
+  xs' /    > n1      xs' /     \ sufm
+     n2                n2       n1
 
    g2 = undo g1 xs xsm           h2 = undo g2 (ys' ++ xs'm) (xs' ++ ys'm)
                                     = undo h1 sufm sufm'  (note: sufm, sufm' are not mirrors)
@@ -2725,8 +2858,8 @@ Section pstore_G.
           |ys'                         ↑ ys'm
           v                            |
     xs'm / <-                        -> <-
-     r2 <    \ sufm'          xs'   /    \ sufm'
-              r1                  r2     r1
+     n2 <    \ sufm'          xs'   /    \ sufm'
+              n1                  n2     n1
 *)
     set h2 := undo_graph h1 sufm sufm'.
 
@@ -2758,7 +2891,7 @@ Section pstore_G.
         by (eapply mirror_mirror; eauto).
       apply undo_iso; eauto; [].
       enough (list_to_set ysm ⊆ h1) by set_solver.
-      apply path_all_in with r1 orig; eauto.
+      apply path_all_in with n1 orig; eauto.
     }
     exists h2.
     constructor; eauto; [].
@@ -2802,18 +2935,18 @@ Section pstore_G.
     }
   Admitted.
 
-  Lemma use_snapshots γ (t0:location) M C G r σ gen :
+  Lemma use_snapshots γ (t0:location) M C G root σ gen :
     meta t0 nroot γ -∗
     snapshots t0 M C G -∗
-    pstore_map_elem γ r σ gen -∗
-    ⌜(r, σ, gen) ∈ C /\ snapshot_inv M C G r σ gen⌝.
+    pstore_map_elem γ root σ gen -∗
+    ⌜(root, σ, gen) ∈ C /\ snapshot_inv M C G root σ gen⌝.
   Proof.
     iIntros "Hmeta [%γ' (%Hsnap&Hmeta'&HC)] Helem".
     iDestruct (meta_agree with "Hmeta' Hmeta") as "->".
     iDestruct (mono_set_elem_valid with "[$][$]") as "%Hrs".
 
     iPureIntro.
-    destruct Hsnap with r σ gen as (σ', (H1 & H2 & H3)); [ auto | ].
+    destruct Hsnap with root σ gen as (σ', (H1 & H2 & H3)); [ auto | ].
     unfold captured.
     eexists; eauto.
   Qed.
@@ -2832,114 +2965,145 @@ Section pstore_G.
     iIntros (Φ) "(HI&Hsnap) HΦ".
     iDestruct "HI" as open_inv.
 
-    iDestruct "Hsnap" as "[%γ [%t0' [%rs [%snap_gen ((%Eq&->)&Hmeta'&Hsnap)]]]]".
+    iDestruct "Hsnap" as "[%γ [%t0' [%snaproot [%snap_gen ((%Eq&->)&Hmeta'&Hsnap)]]]]".
     inversion Eq. subst t0'. clear Eq.
 
-    iDestruct (use_snapshots with "[$][$][$]") as %(HC & σ1 & HMrs &Hincl & Hsnapgen).
+    iDestruct (use_snapshots with "[$][$][$]") as %(HC & σ0 & HMsnaproot &Hincl & Hsnapgen).
 
     wp_rec. iStep 20.
 
     iDestruct (extract_unaliased with "Hg") as "%".
-    destruct_decide (decide (rs=r)).
+    destruct_decide (decide (snaproot=root)).
     { subst.
       wp_load. iStep 4. iModIntro.
-      iExists _,_,_,_,_,_,_,_,_,_. iFrame. iPureIntro. split_and!; eauto.
+      iExists _,_,_,_,_,_,_,_,_,_,_. iFrame. iPureIntro. split_and!; eauto.
       { destruct Hinv as [X1 X2 X3 X4]. constructor; eauto. naive_solver. } }
 
-    assert (rs ∈ vertices g) as Hrs.
-    { destruct Hinv. apply elem_of_dom_2 in HMrs. set_solver. }
+    assert (snaproot ∈ vertices g) as Hsnaproot.
+    { destruct Hinv. apply elem_of_dom_2 in HMsnaproot. set_solver. }
 
-    eapply ti1 in Hrs; eauto. destruct Hrs as (ds,Hrs).
-    inversion Hrs; first congruence. subst. rename a2 into r'. destruct b.
+    eapply ti1 in Hsnaproot; eauto. destruct Hsnaproot as (ds,Hsnaproot).
+    inversion Hsnaproot; first congruence. subst. rename a2 into n. destruct b as (r, (refv, refgen)).
     iDestruct (big_sepS_elem_of_acc with "[$]") as "(?&Hg)"; first done. simpl.
     wp_load. iStep 2. iModIntro.
     iSpecialize ("Hg" with "[$]").
 
-    remember ((rs, (l, v), r') :: bs) as xs.
-    assert (list_to_set xs ⊆ g).
+    remember ((snaproot, (r, (refv, refgen)), n) :: bs) as xs.
+    assert (list_to_set ((snaproot, (r, (refv, refgen)), n) :: bs) ⊆ g) as Hincl1.
     { eauto using path_all_in. }
+    assert (list_to_set xs ⊆ g) as Hincl2.
+    { subst xs; eauto. }
 
     rewrite (union_difference_L (list_to_set xs) g) //.
 
     iDestruct (big_sepS_union with "Hg") as "(Hxs&Hg)"; first set_solver.
-    wp_apply (pstore_reroot_spec with "[Hr Hxs Hσ0]").
-    4:{ eapply path_restrict. done. }
-    2:done.
-    { destruct Hcoh as [_ X]. eapply locations_of_edges_weak; eauto. }
+    wp_apply (pstore_reroot_spec with "[Hroot Hxs Hρv Hρg]").
+    5:{ eapply path_restrict. done. }
+    3:done.
+    { destruct Hcoh as [_ X]. eapply references_in_weak; naive_solver. }
+    { destruct Hcoh; eauto. }
     { eapply acyclic_weak; eauto using ti2. }
-    { iFrame. }
+    { subst xs. iFrame. }
 
-    iIntros "[%ys (%Hundo&?&?&?)]".
-    assert (mirror xs ys) as Hmirror by eauto using undo_mirror.
+    iIntros "[%ys (%Hundo & Hsnaproot & Hnodes & Hρv & Hρg)]".
+    assert (mirror xs ys) as Hmirror by (subst xs; eauto using undo_mirror).
     wp_store. wp_store. iStep. iModIntro.
-    iDestruct (big_sepS_union_2 with "[$][$]") as "Hs".
+    iDestruct (big_sepS_union_2 with "[$][$]") as "Hnodes".
 
-    iDestruct (extract_unaliased with "Hs") as "%".
+    iDestruct (extract_unaliased with "Hnodes") as "%".
 
-    assert (({[(rs, (l, v), r')]} ∪ list_to_set bs) = (list_to_set xs : gset _)) as Hbs.
+    assert (({[(snaproot, (r, (refv, refgen)), n)]} ∪ list_to_set bs)
+            = (list_to_set xs : gset _)) as Hbs.
     { subst xs. reflexivity. }
 
     set g' : graph_store := undo_graph g xs ys.
 
-    iAssert ⌜forall x y, (rs,x,y) ∉ g'⌝%I as "%".
-    { iIntros (???). destruct a. iDestruct (big_sepS_elem_of with "Hs") as "?"; first done.
-      iDestruct (pointsto_ne rs rs with "[$][$]") as "%". congruence. }
+    iAssert ⌜forall x y, (snaproot,x,y) ∉ g'⌝%I as "%".
+    { iIntros (???). destruct a as (r', (v', gen')).
+      iDestruct (big_sepS_elem_of with "Hnodes") as "?"; first done.
+      simpl.
+      iDestruct (pointsto_ne snaproot snaproot with "[$][$]") as "%". congruence. }
 
-    assert (exists h', graph_iso h h' /\ history_inv g' rs h' orig) as (h' & Hiso & Hist').
+    assert (exists h', graph_iso h h' /\ history_inv g' snaproot h' orig) as (h' & Hiso & Hist').
     {
       destruct Hgraph.
       unfold g'.
-      eapply undo_preserves_histo; eauto.
+      subst xs; eapply undo_preserves_histo; eauto.
     }
 
     assert (vertices g' = vertices g) as Hvg.
     { apply mirror_vertices in Hmirror.
       rewrite vertices_union Hmirror -vertices_union -union_difference_L //. }
 
-    assert (σ1 = (apply_diffl (proj2 <$> xs) σ0)).
-    { destruct Hinv as [X1 X2 X3 X4]. eauto. }
+    assert (σ0 = (apply_diffl (vchange_of_edge <$> xs) ρv)).
+    { destruct Hinv as [X1 X2 X3 X4]. subst xs. eauto. }
 
-    assert (rooted_dag g' rs) as Hroot.
-    { eapply undo_preserves_rooted_dag; eauto.
+    assert (rooted_dag g' snaproot) as Hroot.
+    { subst xs; eapply undo_preserves_rooted_dag; eauto.
     - intros k (d, Hk).
-      apply (H5 d k).
-      assumption.
+      apply (H4 d k).
+      unfold g'; assumption.
     }
 
-    iExists t0,rs,orig,(1 + snap_gen),_,g',h',M,_,_. iFrame.
-    iSplitR. 2: iSteps. 1: iPureIntro; split_and!; try done.
+    iExists (* r0, root, orig, gen: *) t0, snaproot, orig, (1 + snap_gen),
+            (* ρv, ρg: *) (apply_diffl (vchange_of_edge <$> xs) ρv),
+                          (apply_diffl (gchange_of_edge <$> xs) ρg),
+            (* g, h: *)   g', h',
+            (* M, C, G: *) M, _, _.
+
+    iFrame.
+    iSplitR.
+    2: {
+      subst xs.
+      iFrame.
+      iSmash.
+    }
+
+    1: iPureIntro; split_and!; try done.
 
     { (* store_inv *)
       destruct Hinv as [X1 X2 X3 X4 X5]. constructor.
       { rewrite X1 Hvg.
-        apply elem_of_dom_2 in X4, HMrs.
-        apply path_ends_vertices in Hrs.
+        apply elem_of_dom_2 in X4, HMsnaproot.
+        apply path_ends_vertices in Hsnaproot.
         set_solver. }
       { set_solver. }
       { set_solver. }
       { set_solver. }
-      { intros. eapply undo_preserves_model; eauto.
-        intros k (d, Hk). apply (H5 d k). eauto. }
+      { subst xs.
+        intros. eapply undo_preserves_model; eauto.
+        intros k (d, Hk). apply (H4 d k). eauto. }
     }
 
     { (* topology_inv *)
-      apply undo_preserves_topo with r; eauto.
-      - { destruct Hinv; eauto. }
+      subst; apply undo_preserves_topo with root; eauto.
+      - destruct Hinv. eauto.
       - unfold captured; eexists _, _; eapply HC.
     }
 
     { (* coherent *)
       destruct Hcoh as [X1 X2]. constructor.
-      { intros ???. rewrite dom_apply_diffl. apply X1 in H7.
-        eapply use_locations_of_edges_in in Hrs. 2:done.
+      { intros ???. rewrite dom_apply_diffl. apply X1 in H6.
+        eapply use_references_in in Hsnaproot. 2:done.
         set_solver.
       } {
+        subst xs.
         rewrite dom_apply_diffl. intros ???? Hedge.
         rewrite /edge elem_of_union in Hedge. rewrite elem_of_union.
         destruct Hedge as [Hedge|Hedge].
-        { right. eauto using undo_same_fst_label. }
-        { left. eapply (X2 r0). eapply elem_of_subseteq. 2:done. set_solver. }
-    } }
+        { right.
+          Check undo_same_fst_label.
+          rewrite -vchange_fst_label.
+          eauto using undo_same_fst_label. }
+        { left. eapply (X2 n0). eapply elem_of_subseteq. 2:done. set_solver. }
+    }
+
+    { (* dom ρv = dom ρg *)
+      do 2 rewrite dom_apply_diffl.
+      rewrite -vchange_fst_label -gchange_fst_label.
+      rewrite coh4. reflexivity.
+    }
+    }
 
     { (* global_gen_inv *)
       constructor.
